Refactoring about Hilbert Deduction System (#154)
* modal

* int

* fx

* `Λ` to `H`

* fx

Foundation/IntProp/ConsistentTableau.lean
@@ -9,7 +9,7 @@ open System FiniteContext
 open Formula
 
 variable {α : Type u}
-variable {Λ : Hilbert α}
+variable {H : Hilbert α}
 
 def Tableau (α : Type u) := Theory α × Theory α
 
@@ -24,7 +24,7 @@ instance : HasSubset (Tableau α) := ⟨λ t₁ t₂ => t₁.1 ⊆ t₂.1 ∧ t�
   . intro h; cases h; simp;
   . rintro ⟨h₁, h₂⟩; cases t₁; cases t₂; simp_all;
 
-def Consistent (Λ : Hilbert α) (t : Tableau α) := ∀ {Γ Δ : List (Formula α)}, (∀ φ ∈ Γ, φ ∈ t.1) → (∀ φ ∈ Δ, φ ∈ t.2) → Λ ⊬ ⋀Γ ➝ ⋁Δ
+def Consistent (H : Hilbert α) (t : Tableau α) := ∀ {Γ Δ : List (Formula α)}, (∀ φ ∈ Γ, φ ∈ t.1) → (∀ φ ∈ Δ, φ ∈ t.2) → H ⊬ ⋀Γ ➝ ⋁Δ
 
 variable {φ ψ: Formula α} {T U : Theory α}
 
@@ -32,16 +32,16 @@ section
 
 variable [DecidableEq α]
 
-lemma iff_consistent_insert₁ : Tableau.Consistent Λ ((insert φ T), U) ↔ ∀ {Γ Δ : List (Formula α)}, (∀ φ ∈ Γ, φ ∈ T) → (∀ φ ∈ Δ, φ ∈ U) → Λ ⊬ φ ⋏ ⋀Γ ➝ ⋁Δ := by
+lemma iff_consistent_insert₁ : Tableau.Consistent H ((insert φ T), U) ↔ ∀ {Γ Δ : List (Formula α)}, (∀ φ ∈ Γ, φ ∈ T) → (∀ φ ∈ Δ, φ ∈ U) → H ⊬ φ ⋏ ⋀Γ ➝ ⋁Δ := by
   constructor;
   . intro h Γ Δ hΓ hΔ;
     by_contra hC;
-    have : Λ ⊬ ⋀(φ :: Γ) ➝ ⋁Δ := h (by simp; intro ψ hq; right; exact hΓ ψ hq;) hΔ;
-    have : Λ ⊢! ⋀(φ :: Γ) ➝ ⋁Δ := iff_imply_left_cons_conj'!.mpr hC;
+    have : H ⊬ ⋀(φ :: Γ) ➝ ⋁Δ := h (by simp; intro ψ hq; right; exact hΓ ψ hq;) hΔ;
+    have : H ⊢! ⋀(φ :: Γ) ➝ ⋁Δ := iff_imply_left_cons_conj'!.mpr hC;
     contradiction;
   . intro h Γ Δ hΓ hΔ;
     simp_all only [Set.mem_insert_iff];
-    have : Λ ⊬ φ ⋏ ⋀(Γ.remove φ) ➝ ⋁Δ := h (by
+    have : H ⊬ φ ⋏ ⋀(Γ.remove φ) ➝ ⋁Δ := h (by
       intro ψ hq;
       have := by simpa using hΓ ψ $ List.mem_of_mem_remove hq;
       cases this with
@@ -49,26 +49,26 @@ lemma iff_consistent_insert₁ : Tableau.Consistent Λ ((insert φ T), U) ↔ �
       | inr h => assumption;
     ) hΔ;
     by_contra hC;
-    have : Λ ⊢! φ ⋏ ⋀(Γ.remove φ) ➝ ⋁Δ := imp_trans''! and_comm! $ imply_left_remove_conj! (φ := φ) hC;
+    have : H ⊢! φ ⋏ ⋀(Γ.remove φ) ➝ ⋁Δ := imp_trans''! and_comm! $ imply_left_remove_conj! (φ := φ) hC;
     contradiction;
 
-lemma iff_not_consistent_insert₁ : ¬Tableau.Consistent Λ ((insert φ T), U) ↔ ∃ Γ Δ : List (Formula α), (∀ φ ∈ Γ, φ ∈ T) ∧ (∀ φ ∈ Δ, φ ∈ U) ∧ Λ ⊢! φ ⋏ ⋀Γ ➝ ⋁Δ := by
+lemma iff_not_consistent_insert₁ : ¬Tableau.Consistent H ((insert φ T), U) ↔ ∃ Γ Δ : List (Formula α), (∀ φ ∈ Γ, φ ∈ T) ∧ (∀ φ ∈ Δ, φ ∈ U) ∧ H ⊢! φ ⋏ ⋀Γ ➝ ⋁Δ := by
   constructor;
   . contrapose; push_neg; apply iff_consistent_insert₁.mpr;
   . contrapose; push_neg; apply iff_consistent_insert₁.mp;
 
-variable [Λ.IncludeEFQ]
+variable [H.IncludeEFQ]
 
-lemma iff_consistent_insert₂ : Tableau.Consistent Λ (T, (insert φ U)) ↔ ∀ {Γ Δ : List (Formula α)}, (∀ φ ∈ Γ, φ ∈ T) → (∀ φ ∈ Δ, φ ∈ U) → Λ ⊬ ⋀Γ ➝ φ ⋎ ⋁Δ := by
+lemma iff_consistent_insert₂ : Tableau.Consistent H (T, (insert φ U)) ↔ ∀ {Γ Δ : List (Formula α)}, (∀ φ ∈ Γ, φ ∈ T) → (∀ φ ∈ Δ, φ ∈ U) → H ⊬ ⋀Γ ➝ φ ⋎ ⋁Δ := by
   constructor;
   . intro h Γ Δ hΓ hΔ;
     by_contra hC;
-    have : Λ ⊬ ⋀Γ ➝ ⋁(φ :: Δ) := h hΓ (by simp; intro ψ hq; right; exact hΔ ψ hq);
-    have : Λ ⊢! ⋀Γ ➝ ⋁(φ :: Δ) := implyRight_cons_disj!.mpr hC;
+    have : H ⊬ ⋀Γ ➝ ⋁(φ :: Δ) := h hΓ (by simp; intro ψ hq; right; exact hΔ ψ hq);
+    have : H ⊢! ⋀Γ ➝ ⋁(φ :: Δ) := implyRight_cons_disj!.mpr hC;
     contradiction;
   . intro h Γ Δ hΓ hΔ;
     simp_all;
-    have : Λ ⊬ ⋀Γ ➝ φ ⋎ ⋁(Δ.remove φ) := h hΓ (by
+    have : H ⊬ ⋀Γ ➝ φ ⋎ ⋁(Δ.remove φ) := h hΓ (by
       intro ψ hq;
       have := by simpa using hΔ ψ $ List.mem_of_mem_remove hq;
       cases this with
@@ -76,11 +76,11 @@ lemma iff_consistent_insert₂ : Tableau.Consistent Λ (T, (insert φ U)) ↔ �
       | inr h => assumption;
     );
     by_contra hC;
-    have : Λ ⊢! ⋀Γ ➝ φ ⋎ ⋁(Δ.remove φ) := imp_trans''! hC $ forthback_disj_remove;
+    have : H ⊢! ⋀Γ ➝ φ ⋎ ⋁(Δ.remove φ) := imp_trans''! hC $ forthback_disj_remove;
     contradiction;
 
 
-lemma iff_not_consistent_insert₂ : ¬Tableau.Consistent Λ (T, (insert φ U)) ↔ ∃ Γ Δ : List (Formula α), (∀ φ ∈ Γ, φ ∈ T) ∧ (∀ φ ∈ Δ, φ ∈ U) ∧ Λ ⊢! ⋀Γ ➝ φ ⋎ ⋁Δ := by
+lemma iff_not_consistent_insert₂ : ¬Tableau.Consistent H (T, (insert φ U)) ↔ ∃ Γ Δ : List (Formula α), (∀ φ ∈ Γ, φ ∈ T) ∧ (∀ φ ∈ Δ, φ ∈ U) ∧ H ⊢! ⋀Γ ➝ φ ⋎ ⋁Δ := by
   constructor;
   . contrapose; push_neg; apply iff_consistent_insert₂.mpr;
   . contrapose; push_neg; apply iff_consistent_insert₂.mp;
@@ -89,7 +89,7 @@ section Consistent
 
 variable {t : Tableau α}
 
-lemma consistent_either (hCon : Tableau.Consistent Λ t) (φ : Formula α) : Tableau.Consistent Λ ((insert φ t.1), t.2) ∨ Tableau.Consistent Λ (t.1, (insert φ t.2)) := by
+lemma consistent_either (hCon : Tableau.Consistent H t) (φ : Formula α) : Tableau.Consistent H ((insert φ t.1), t.2) ∨ Tableau.Consistent H (t.1, (insert φ t.2)) := by
   by_contra hC;
   push_neg at hC;
   have ⟨hC₁, hC₂⟩ := hC;
@@ -99,27 +99,27 @@ lemma consistent_either (hCon : Tableau.Consistent Λ t) (φ : Formula α) : Tab
 
   obtain ⟨Γ₂, Δ₂, hΓ₂, hΔ₂, h₂⟩ := iff_not_consistent_insert₂.mp hC₂;
 
-  have : Λ ⊢! ⋀(Γ₁ ++ Γ₂) ➝ ⋁(Δ₁ ++ Δ₂) := imp_trans''! (and₁'! iff_concat_conj!) $ imp_trans''! (cut! h₁ h₂) (and₂'! iff_concact_disj!);
-  have : Λ ⊬ ⋀(Γ₁ ++ Γ₂) ➝ ⋁(Δ₁ ++ Δ₂) := hCon (by simp; rintro ψ (hq₁ | hq₂); exact hΓ₁ ψ hq₁; exact hΓ₂ ψ hq₂) (by simp; rintro ψ (hq₁ | hq₂); exact hΔ₁ ψ hq₁; exact hΔ₂ ψ hq₂);
+  have : H ⊢! ⋀(Γ₁ ++ Γ₂) ➝ ⋁(Δ₁ ++ Δ₂) := imp_trans''! (and₁'! iff_concat_conj!) $ imp_trans''! (cut! h₁ h₂) (and₂'! iff_concact_disj!);
+  have : H ⊬ ⋀(Γ₁ ++ Γ₂) ➝ ⋁(Δ₁ ++ Δ₂) := hCon (by simp; rintro ψ (hq₁ | hq₂); exact hΓ₁ ψ hq₁; exact hΓ₂ ψ hq₂) (by simp; rintro ψ (hq₁ | hq₂); exact hΔ₁ ψ hq₁; exact hΔ₂ ψ hq₂);
   contradiction;
 
-omit [DecidableEq α] [Λ.IncludeEFQ] in
-lemma disjoint_of_consistent (hCon : Tableau.Consistent Λ t) : Disjoint t.1 t.2 := by
+omit [DecidableEq α] [H.IncludeEFQ] in
+lemma disjoint_of_consistent (hCon : Tableau.Consistent H t) : Disjoint t.1 t.2 := by
   by_contra h;
   obtain ⟨T, hp₁, hp₂, hp⟩ := by simpa [Disjoint] using h;
   obtain ⟨φ, hp⟩ := Set.nonempty_def.mp $ Set.nonempty_iff_ne_empty.mpr hp;
   simp [Consistent] at hCon;
-  have : Λ ⊬ ⋀[φ] ➝ ⋁[φ] := hCon
+  have : H ⊬ ⋀[φ] ➝ ⋁[φ] := hCon
     (by simp_all; apply hp₁; assumption)
     (by simp_all; apply hp₂; assumption);
-  have : Λ ⊢! ⋀[φ] ➝ ⋁[φ] := by simp;
+  have : H ⊢! ⋀[φ] ➝ ⋁[φ] := by simp;
   contradiction;
 
-omit [DecidableEq α] [Λ.IncludeEFQ] in
-lemma not_mem₂ (hCon : Tableau.Consistent Λ t) {Γ : List (Formula α)} (hΓ : ∀ φ ∈ Γ, φ ∈ t.1) (h : Λ ⊢! ⋀Γ ➝ ψ) : ψ ∉ t.2 := by
+omit [DecidableEq α] [H.IncludeEFQ] in
+lemma not_mem₂ (hCon : Tableau.Consistent H t) {Γ : List (Formula α)} (hΓ : ∀ φ ∈ Γ, φ ∈ t.1) (h : H ⊢! ⋀Γ ➝ ψ) : ψ ∉ t.2 := by
   by_contra hC;
-  have : Λ ⊢! ⋀Γ ➝ ⋁[ψ] := by simpa;
-  have : Λ ⊬ ⋀Γ ➝ ⋁[ψ] := hCon (by aesop) (by aesop);
+  have : H ⊢! ⋀Γ ➝ ⋁[ψ] := by simpa;
+  have : H ⊬ ⋀Γ ➝ ⋁[ψ] := hCon (by aesop) (by aesop);
   contradiction;
 
 end Consistent
@@ -146,19 +146,19 @@ lemma mem₁_of_not_mem₂ (hMat : Saturated t) : φ ∉ t.2 → φ ∈ t.1 := b
   | inr h' => exact absurd h' h;
 
 
-lemma not_mem₁_iff_mem₂ (hCon : Tableau.Consistent Λ t) (hMat : Saturated t) : φ ∉ t.1 ↔ φ ∈ t.2 := by
+lemma not_mem₁_iff_mem₂ (hCon : Tableau.Consistent H t) (hMat : Saturated t) : φ ∉ t.1 ↔ φ ∈ t.2 := by
   constructor;
   . apply mem₂_of_not_mem₁ hMat;
   . apply Set.disjoint_right.mp $ disjoint_of_consistent hCon;
 
-lemma not_mem₂_iff_mem₁ (hCon : Tableau.Consistent Λ t) (hMat : Saturated t) : φ ∉ t.2 ↔ φ ∈ t.1 := by
+lemma not_mem₂_iff_mem₁ (hCon : Tableau.Consistent H t) (hMat : Saturated t) : φ ∉ t.2 ↔ φ ∈ t.1 := by
   constructor;
   . apply mem₁_of_not_mem₂ hMat;
   . apply Set.disjoint_left.mp $ disjoint_of_consistent hCon;
 
 lemma saturated_duality
   {t₁ t₂ : Tableau α}
-  (ct₁ : Tableau.Consistent Λ t₁) (ct₂ : Tableau.Consistent Λ t₂)
+  (ct₁ : Tableau.Consistent H t₁) (ct₂ : Tableau.Consistent H t₂)
   (st₁ : Saturated t₁) (st₂ : Saturated t₂)
   : t₁.1 = t₂.1 ↔ t₁.2 = t₂.2 := by
   constructor;
@@ -181,79 +181,80 @@ lemma saturated_duality
 
 end Saturated
 
-variable [Λ.IncludeEFQ]
+variable [H.IncludeEFQ]
 
-lemma self_consistent [h : System.Consistent Λ] : Tableau.Consistent Λ (Ax(Λ), ∅) := by
+lemma self_consistent [h : System.Consistent H] : Tableau.Consistent H (H.axioms, ∅) := by
   intro Γ Δ hΓ hΔ;
   replace hΔ : Δ = [] := List.nil_iff.mpr hΔ;
   obtain ⟨ψ, hq⟩ := h.exists_unprovable;
   by_contra hC;
-  have : Λ ⊢! ψ := by
+  have : H ⊢! ψ := by
     subst hΔ;
     simp at hC;
     exact imp_trans''! hC efq! ⨀ (by
       apply iff_provable_list_conj.mpr;
-      exact λ _ hp => ⟨Deduction.eaxm $ hΓ _ hp⟩;
+      intro φ hφ;
+      exact Hilbert.Deduction.eaxm! $ hΓ _ hφ;
     );
   contradiction;
 
 section lindenbaum
 
 variable [Encodable α]
-variable (Λ)
+variable (H)
 variable {t : Tableau α}
 
 open Classical
 open Encodable
 
-def lindenbaum_next (φ : Formula α) (t : Tableau α) : Tableau α := if Tableau.Consistent Λ (insert φ t.1, t.2) then (insert φ t.1, t.2) else (t.1, insert φ t.2)
+def lindenbaum_next (φ : Formula α) (t : Tableau α) : Tableau α := if Tableau.Consistent H (insert φ t.1, t.2) then (insert φ t.1, t.2) else (t.1, insert φ t.2)
 
 def lindenbaum_next_indexed [Encodable α] (t : Tableau α) : ℕ → Tableau α
   | 0 => t
   | i + 1 =>
     match (decode i) with
-    | some φ => (lindenbaum_next_indexed t i).lindenbaum_next Λ φ
+    | some φ => (lindenbaum_next_indexed t i).lindenbaum_next H φ
     | none => lindenbaum_next_indexed t i
-local notation:max t"[" i "]" => lindenbaum_next_indexed Λ t i
+local notation:max t"[" i "]" => lindenbaum_next_indexed H t i
 
 def lindenbaum_maximal (t : Tableau α) : Tableau α := (⋃ i, t[i].1, ⋃ i, t[i].2)
-local notation:max t"∞" => lindenbaum_maximal Λ t
+local notation:max t"∞" => lindenbaum_maximal H t
 
-variable {Λ}
+variable {H}
 
 omit [Encodable α] in
-lemma next_parametericConsistent (consistent : Tableau.Consistent Λ t) (φ : Formula α) : Tableau.Consistent Λ (t.lindenbaum_next Λ φ) := by
+lemma next_parametericConsistent (consistent : Tableau.Consistent H t) (φ : Formula α) : Tableau.Consistent H (t.lindenbaum_next H φ) := by
   simp [lindenbaum_next];
   split;
   . simpa;
   . have := consistent_either consistent φ;
     simp_all only [false_or];
 
-omit [Λ.IncludeEFQ] in
+omit [H.IncludeEFQ] in
 @[simp]
-lemma lindenbaum_next_indexed_zero {t : Tableau α} : (t.lindenbaum_next_indexed Λ 0) = t := by simp [lindenbaum_next_indexed]
+lemma lindenbaum_next_indexed_zero {t : Tableau α} : (t.lindenbaum_next_indexed H 0) = t := by simp [lindenbaum_next_indexed]
 
-lemma lindenbaum_next_indexed_parametricConsistent_succ {i : ℕ} : Tableau.Consistent Λ t[i] → Tableau.Consistent Λ t[i + 1] := by
+lemma lindenbaum_next_indexed_parametricConsistent_succ {i : ℕ} : Tableau.Consistent H t[i] → Tableau.Consistent H t[i + 1] := by
   simp [lindenbaum_next_indexed];
   split;
   . intro h; apply next_parametericConsistent; assumption;
   . tauto;
 
-omit [Λ.IncludeEFQ] in
+omit [H.IncludeEFQ] in
 lemma mem_lindenbaum_next_indexed (t) (φ : Formula α) : φ ∈ t[(encode φ) + 1].1 ∨ φ ∈ t[(encode φ) + 1].2 := by
   simp [lindenbaum_next_indexed, lindenbaum_next];
   split;
   . left; tauto;
   . right; tauto;
 
-lemma lindenbaum_next_indexed_parametricConsistent (consistent : Tableau.Consistent Λ t) (i : ℕ) : Tableau.Consistent Λ t[i] := by
+lemma lindenbaum_next_indexed_parametricConsistent (consistent : Tableau.Consistent H t) (i : ℕ) : Tableau.Consistent H t[i] := by
   induction i with
   | zero => simpa;
   | succ i ih => apply lindenbaum_next_indexed_parametricConsistent_succ; assumption;
 
 variable {m n : ℕ}
 
-omit [Λ.IncludeEFQ] in
+omit [H.IncludeEFQ] in
 lemma lindenbaum_next_indexed_subset₁_of_lt (h : m ≤ n) : t[m].1 ⊆ t[n].1 := by
   induction h with
   | refl => simp;
@@ -263,7 +264,7 @@ lemma lindenbaum_next_indexed_subset₁_of_lt (h : m ≤ n) : t[m].1 ⊆ t[n].1 
     . split <;> tauto;
     . tauto;
 
-omit [Λ.IncludeEFQ] in
+omit [H.IncludeEFQ] in
 lemma lindenbaum_next_indexed_subset₂_of_lt (h : m ≤ n) : t[m].2 ⊆ t[n].2 := by
   induction h with
   | refl => simp;
@@ -273,7 +274,7 @@ lemma lindenbaum_next_indexed_subset₂_of_lt (h : m ≤ n) : t[m].2 ⊆ t[n].2 
     . split <;> tauto;
     . tauto;
 
-lemma exists_parametricConsistent_saturated_tableau (hCon : Tableau.Consistent Λ t) : ∃ u, t ⊆ u ∧ (Tableau.Consistent Λ u) ∧ (Saturated u) := by
+lemma exists_parametricConsistent_saturated_tableau (hCon : Tableau.Consistent H t) : ∃ u, t ⊆ u ∧ (Tableau.Consistent H u) ∧ (Saturated u) := by
   use t∞;
   refine ⟨?subset, ?consistent, ?saturated⟩;
   case subset => constructor <;> apply Set.subset_iUnion_of_subset 0 (by simp);
@@ -323,10 +324,10 @@ end Tableau
 
 open Tableau
 
-structure SaturatedConsistentTableau (Λ : Hilbert α) where
+structure SaturatedConsistentTableau (H : Hilbert α) where
   tableau : Tableau α
   saturated : Saturated tableau
-  consistent : Tableau.Consistent Λ tableau
+  consistent : Tableau.Consistent H tableau
 
 alias SCT := SaturatedConsistentTableau
 
@@ -334,13 +335,13 @@ namespace SaturatedConsistentTableau
 
 variable {t₀ : Tableau α} {φ ψ : Formula α}
 
-lemma lindenbaum [Λ.IncludeEFQ] [Encodable α] (hCon : Tableau.Consistent Λ t₀) : ∃ (t : SaturatedConsistentTableau Λ), t₀ ⊆ t.tableau := by
+lemma lindenbaum [H.IncludeEFQ] [Encodable α] (hCon : Tableau.Consistent H t₀) : ∃ (t : SaturatedConsistentTableau H), t₀ ⊆ t.tableau := by
   obtain ⟨t, ht, hCon, hMax⟩ := Tableau.lindenbaum hCon;
   exact ⟨⟨t, hMax, hCon⟩, ht⟩;
 
-instance [System.Consistent Λ] [Λ.IncludeEFQ] [Encodable α] : Nonempty (SCT Λ) := ⟨lindenbaum Tableau.self_consistent |>.choose⟩
+instance [System.Consistent H] [H.IncludeEFQ] [Encodable α] : Nonempty (SCT H) := ⟨lindenbaum Tableau.self_consistent |>.choose⟩
 
-variable {t : SCT Λ}
+variable {t : SCT H}
 
 @[simp] lemma disjoint : Disjoint t.tableau.1 t.tableau.2 := t.tableau.disjoint_of_consistent t.consistent
 
@@ -348,7 +349,7 @@ lemma not_mem₁_iff_mem₂ : φ ∉ t.tableau.1 ↔ φ ∈ t.tableau.2 := Table
 
 lemma not_mem₂_iff_mem₁ : φ ∉ t.tableau.2 ↔ φ ∈ t.tableau.1 := Tableau.not_mem₂_iff_mem₁ t.consistent t.saturated
 
-variable {t t₁ t₂ : SCT Λ}
+variable {t t₁ t₂ : SCT H}
 
 lemma saturated_duality: t₁.tableau.1 = t₂.tableau.1 ↔ t₁.tableau.2 = t₂.tableau.2 := Tableau.saturated_duality t₁.consistent t₂.consistent t₁.saturated t₂.saturated
 
@@ -361,27 +362,27 @@ lemma equality_of₁ (e₁ : t₁.tableau.1 = t₂.tableau.1) : t₁ = t₂ := b
 
 lemma equality_of₂ (e₂ : t₁.tableau.2 = t₂.tableau.2) : t₁ = t₂ := equality_of₁ $ saturated_duality.mpr e₂
 
-lemma not_mem₂ {Γ : List (Formula α)} (hΓ : ∀ φ ∈ Γ, φ ∈ t.tableau.1) (h : Λ ⊢! ⋀Γ ➝ ψ) : ψ ∉ t.tableau.2 := t.tableau.not_mem₂ t.consistent hΓ h
+lemma not_mem₂ {Γ : List (Formula α)} (hΓ : ∀ φ ∈ Γ, φ ∈ t.tableau.1) (h : H ⊢! ⋀Γ ➝ ψ) : ψ ∉ t.tableau.2 := t.tableau.not_mem₂ t.consistent hΓ h
 
-lemma mdp₁ (hp₁ : φ ∈ t.tableau.1) (h : Λ ⊢! φ ➝ ψ) : ψ ∈ t.tableau.1 := by
+lemma mdp₁ (hp₁ : φ ∈ t.tableau.1) (h : H ⊢! φ ➝ ψ) : ψ ∈ t.tableau.1 := by
   apply not_mem₂_iff_mem₁.mp;
   by_contra hq₂;
-  have : Λ ⊬ φ ➝ ψ := by simpa using t.consistent (Γ := [φ]) (Δ := [ψ]) (by simpa) (by simpa);
+  have : H ⊬ φ ➝ ψ := by simpa using t.consistent (Γ := [φ]) (Δ := [ψ]) (by simpa) (by simpa);
   contradiction;
 
 @[simp]
 lemma mem₁_verum : ⊤ ∈ t.tableau.1 := by
   apply not_mem₂_iff_mem₁.mp;
   by_contra hC;
-  have : Λ ⊬ ⋀[] ➝ ⋁[⊤] := t.consistent (by simp) (by simpa);
-  have : Λ ⊢! ⋀[] ➝ ⋁[⊤] := by simp;
+  have : H ⊬ ⋀[] ➝ ⋁[⊤] := t.consistent (by simp) (by simpa);
+  have : H ⊢! ⋀[] ➝ ⋁[⊤] := by simp;
   contradiction;
 
 @[simp]
 lemma not_mem₁_falsum : ⊥ ∉ t.tableau.1 := by
   by_contra hC;
-  have : Λ ⊬ ⋀[⊥] ➝ ⋁[] := t.consistent (by simpa) (by simp);
-  have : Λ ⊢! ⋀[⊥] ➝ ⋁[] := by simp;
+  have : H ⊬ ⋀[⊥] ➝ ⋁[] := t.consistent (by simpa) (by simp);
+  have : H ⊢! ⋀[⊥] ➝ ⋁[] := by simp;
   contradiction;
 
 @[simp]
@@ -391,8 +392,8 @@ lemma iff_mem₁_and : φ ⋏ ψ ∈ t.tableau.1 ↔ φ ∈ t.tableau.1 ∧ ψ �
   . rintro ⟨hp, hq⟩;
     apply not_mem₂_iff_mem₁.mp;
     by_contra hC;
-    have : Λ ⊢! ⋀[φ, ψ] ➝ ⋁[φ ⋏ ψ] := by simp;
-    have : Λ ⊬ ⋀[φ, ψ] ➝ ⋁[φ ⋏ ψ] := t.consistent (by simp_all) (by simp_all);
+    have : H ⊢! ⋀[φ, ψ] ➝ ⋁[φ ⋏ ψ] := by simp;
+    have : H ⊬ ⋀[φ, ψ] ➝ ⋁[φ ⋏ ψ] := t.consistent (by simp_all) (by simp_all);
     contradiction;
 
 lemma iff_mem₁_conj {Γ : List (Formula α)} : ⋀Γ ∈ t.tableau.1 ↔ ∀ φ ∈ Γ, φ ∈ t.tableau.1 := by
@@ -416,8 +417,8 @@ lemma iff_mem₁_or : φ ⋎ ψ ∈ t.tableau.1 ↔ φ ∈ t.tableau.1 ∨ ψ �
     by_contra hC; push_neg at hC;
     have : φ ∈ t.tableau.2 := not_mem₁_iff_mem₂.mp hC.1;
     have : ψ ∈ t.tableau.2 := not_mem₁_iff_mem₂.mp hC.2;
-    have : Λ ⊢! ⋀[φ ⋎ ψ] ➝ ⋁[φ, ψ] := by simp;
-    have : Λ ⊬ ⋀[φ ⋎ ψ] ➝ ⋁[φ, ψ] := t.consistent (by simp_all) (by simp_all);
+    have : H ⊢! ⋀[φ ⋎ ψ] ➝ ⋁[φ, ψ] := by simp;
+    have : H ⊬ ⋀[φ ⋎ ψ] ➝ ⋁[φ, ψ] := t.consistent (by simp_all) (by simp_all);
     contradiction;
   . intro h;
     cases h with
@@ -436,15 +437,15 @@ lemma mem₂_neg_of_mem₁ [DecidableEq α] : φ ∈ t.tableau.1 → ∼φ ∈ t
   intro h;
   exact not_mem₁_iff_mem₂ (φ := ∼φ) (t := t) |>.mp $ not_mem₁_neg_of_mem₁ h;
 
-lemma mem₁_of_provable : Λ ⊢! φ → φ ∈ t.tableau.1 := by
+lemma mem₁_of_provable : H ⊢! φ → φ ∈ t.tableau.1 := by
   intro h;
   exact mdp₁ mem₁_verum $ imply₁'! h;
 
 lemma mdp₁_mem [DecidableEq α] (hp : φ ∈ t.tableau.1) (h : φ ➝ ψ ∈ t.tableau.1) : ψ ∈ t.tableau.1 := by
   apply not_mem₂_iff_mem₁.mp;
   by_contra hC;
-  have : Λ ⊬ (φ ⋏ (φ ➝ ψ)) ➝ ψ := t.consistent (Γ := [φ, φ ➝ ψ]) (Δ := [ψ]) (by aesop) (by simpa);
-  have : Λ ⊢! (φ ⋏ (φ ➝ ψ)) ➝ ψ := mdp_in!
+  have : H ⊬ (φ ⋏ (φ ➝ ψ)) ➝ ψ := t.consistent (Γ := [φ, φ ➝ ψ]) (Δ := [ψ]) (by aesop) (by simpa);
+  have : H ⊢! (φ ⋏ (φ ➝ ψ)) ➝ ψ := mdp_in!
   contradiction;
 
 end SaturatedConsistentTableau
