Foundation/IntProp/Deduction.lean
@@ -7,44 +7,49 @@ namespace LO.IntProp
 variable {α : Type u}
 
 structure Hilbert (α) where
-  axiomSet : Theory α
-notation "Ax(" Λ ")" => Hilbert.axiomSet Λ
+  axioms : Theory α
 
 namespace Hilbert
 
-class IncludeEFQ (Λ : Hilbert α) where
-  include_EFQ : 𝗘𝗙𝗤 ⊆ Ax(Λ) := by simp
+variable {H : Hilbert α}
 
-class IncludeLEM (Λ : Hilbert α) where
-  include_LEM : 𝗟𝗘𝗠 ⊆ Ax(Λ) := by simp
 
-class IncludeDNE (Λ : Hilbert α) where
-  include_DNE : 𝗗𝗡𝗘 ⊆ Ax(Λ) := by simp
+section
 
-end Hilbert
+class IncludeEFQ (H : Hilbert α) where
+  include_EFQ : 𝗘𝗙𝗤 ⊆ H.axioms := by simp
 
-inductive Deduction (Λ : Hilbert α) : Formula α → Type _
-  | eaxm {φ}     : φ ∈ Ax(Λ) → Deduction Λ φ
-  | mdp {φ ψ}    : Deduction Λ (φ ➝ ψ) → Deduction Λ φ → Deduction Λ ψ
-  | verum        : Deduction Λ $ ⊤
-  | imply₁ φ ψ   : Deduction Λ $ φ ➝ ψ ➝ φ
-  | imply₂ φ ψ χ : Deduction Λ $ (φ ➝ ψ ➝ χ) ➝ (φ ➝ ψ) ➝ φ ➝ χ
-  | and₁ φ ψ     : Deduction Λ $ φ ⋏ ψ ➝ φ
-  | and₂ φ ψ     : Deduction Λ $ φ ⋏ ψ ➝ ψ
-  | and₃ φ ψ     : Deduction Λ $ φ ➝ ψ ➝ φ ⋏ ψ
-  | or₁ φ ψ      : Deduction Λ $ φ ➝ φ ⋎ ψ
-  | or₂ φ ψ      : Deduction Λ $ ψ ➝ φ ⋎ ψ
-  | or₃ φ ψ χ    : Deduction Λ $ (φ ➝ χ) ➝ (ψ ➝ χ) ➝ (φ ⋎ ψ ➝ χ)
-  | neg_equiv φ  : Deduction Λ $ Axioms.NegEquiv φ
+class IncludeLEM (H : Hilbert α) where
+  include_LEM : 𝗟𝗘𝗠 ⊆ H.axioms := by simp
+
+class IncludeDNE (H : Hilbert α) where
+  include_DNE : 𝗗𝗡𝗘 ⊆ H.axioms := by simp
+
+end
+
+
+inductive Deduction (H : Hilbert α) : Formula α → Type _
+  | eaxm {φ}     : φ ∈ H.axioms → Deduction H φ
+  | mdp {φ ψ}    : Deduction H (φ ➝ ψ) → Deduction H φ → Deduction H ψ
+  | verum        : Deduction H $ ⊤
+  | imply₁ φ ψ   : Deduction H $ φ ➝ ψ ➝ φ
+  | imply₂ φ ψ χ : Deduction H $ (φ ➝ ψ ➝ χ) ➝ (φ ➝ ψ) ➝ φ ➝ χ
+  | and₁ φ ψ     : Deduction H $ φ ⋏ ψ ➝ φ
+  | and₂ φ ψ     : Deduction H $ φ ⋏ ψ ➝ ψ
+  | and₃ φ ψ     : Deduction H $ φ ➝ ψ ➝ φ ⋏ ψ
+  | or₁ φ ψ      : Deduction H $ φ ➝ φ ⋎ ψ
+  | or₂ φ ψ      : Deduction H $ ψ ➝ φ ⋎ ψ
+  | or₃ φ ψ χ    : Deduction H $ (φ ➝ χ) ➝ (ψ ➝ χ) ➝ (φ ⋎ ψ ➝ χ)
+  | neg_equiv φ  : Deduction H $ Axioms.NegEquiv φ
 
 instance : System (Formula α) (Hilbert α) := ⟨Deduction⟩
 
 open Deduction
 open Hilbert
 
-variable {Λ : Hilbert α}
+section
 
-instance : System.Minimal Λ where
+instance : System.Minimal H where
   mdp := mdp
   verum := verum
   imply₁ := imply₁
@@ -57,77 +62,84 @@ instance : System.Minimal Λ where
   or₃ := or₃
   neg_equiv := neg_equiv
 
-instance [Λ.IncludeEFQ] : System.HasAxiomEFQ Λ where
+instance [H.IncludeEFQ] : System.HasAxiomEFQ H where
   efq _ := eaxm $ Set.mem_of_subset_of_mem IncludeEFQ.include_EFQ (by simp);
 
-instance [Λ.IncludeLEM] : System.HasAxiomLEM Λ where
+instance [H.IncludeLEM] : System.HasAxiomLEM H where
   lem _ := eaxm $ Set.mem_of_subset_of_mem IncludeLEM.include_LEM (by simp);
 
-instance [Λ.IncludeDNE] : System.HasAxiomDNE Λ where
+instance [H.IncludeDNE] : System.HasAxiomDNE H where
   dne _ := eaxm $ Set.mem_of_subset_of_mem IncludeDNE.include_DNE (by simp);
 
-instance [Λ.IncludeEFQ] : System.Intuitionistic Λ where
+instance [H.IncludeEFQ] : System.Intuitionistic H where
 
-instance [Λ.IncludeDNE] : System.Classical Λ where
+instance [H.IncludeDNE] : System.Classical H where
 
-instance [DecidableEq α] [Λ.IncludeEFQ] [Λ.IncludeLEM] : System.Classical Λ where
+instance [DecidableEq α] [H.IncludeEFQ] [H.IncludeLEM] : System.Classical H where
 
-lemma Deduction.eaxm! {Λ : Hilbert α} {φ : Formula α} (h : φ ∈ Ax(Λ)) : Λ ⊢! φ := ⟨eaxm h⟩
+end
 
 
-namespace Hilbert
+abbrev theorems (H : Hilbert α) : Set (Formula α) := System.theory H
 
-abbrev theorems (Λ : Hilbert α) : Set (Formula α) := System.theory Λ
+
+section systems
+
+variable (α)
 
 protected abbrev Minimal : Hilbert α := ⟨∅⟩
 
-protected abbrev Intuitionistic : Hilbert α := ⟨𝗘𝗙𝗤⟩
-notation "𝐈𝐧𝐭" => Hilbert.Intuitionistic
-instance : IncludeEFQ (α := α) 𝐈𝐧𝐭 where
-instance : System.Intuitionistic (𝐈𝐧𝐭 : Hilbert α) where
+protected abbrev Int : Hilbert α := ⟨𝗘𝗙𝗤⟩
+instance : IncludeEFQ (Hilbert.Int α) where
+instance : System.Intuitionistic (Hilbert.Int α) where
 
-protected abbrev Classical : Hilbert α := ⟨𝗘𝗙𝗤 ∪ 𝗟𝗘𝗠⟩
-notation "𝐂𝐥" => Hilbert.Classical
-instance : IncludeLEM (α := α) 𝐂𝐥 where
-instance : IncludeEFQ (α := α) 𝐂𝐥 where
+protected abbrev Cl : Hilbert α := ⟨𝗘𝗙𝗤 ∪ 𝗟𝗘𝗠⟩
+instance : IncludeLEM (α := α) (Hilbert.Cl α) where
+instance : IncludeEFQ (α := α) (Hilbert.Cl α) where
 
--- `𝐊𝐂` from chagrov & zakharyaschev (1997)
+/--
+  `KC` from Chagrov & Zakharyaschev (1997)
+-/
 protected abbrev KC : Hilbert α := ⟨𝗘𝗙𝗤 ∪ 𝗪𝗟𝗘𝗠⟩
-notation "𝐊𝐂" => Hilbert.KC
-instance : IncludeEFQ (α := α) 𝐊𝐂 where
-instance : System.HasAxiomWeakLEM (𝐊𝐂 : Hilbert α) where
+instance : IncludeEFQ (α := α) (Hilbert.KC α) where
+instance : System.HasAxiomWeakLEM (Hilbert.KC α) where
   wlem φ := by apply eaxm; aesop;
 
--- `𝐋𝐂` from chagrov & zakharyaschev (1997)
+/--
+  `LC` from Chagrov & Zakharyaschev (1997)
+-/
 protected abbrev LC : Hilbert α := ⟨𝗘𝗙𝗤 ∪ 𝗗𝘂𝗺⟩
-notation "𝐋𝐂" => Hilbert.LC
-instance : IncludeEFQ (α := α) 𝐋𝐂 where
-instance : System.HasAxiomDummett (𝐋𝐂 : Hilbert α) where
+instance : IncludeEFQ (α := α) (Hilbert.LC α) where
+instance : System.HasAxiomDummett (Hilbert.LC α) where
   dummett φ ψ := by apply eaxm; aesop;
 
-/- MEMO:
-  Term `WeakMinimal` and `WeakClassical` are from Ariola (2007)
-  Minimal <ₛ WeakMinimal <ₛ WeakClassical <ₛ Classical
--/
+-- MEMO: Minimal <ₛ WeakMinimal <ₛ WeakClassical <ₛ Classical
 
+/--
+  `WeakMinimal` from Ariola (2007)
+-/
 protected abbrev WeakMinimal : Hilbert α := ⟨𝗟𝗘𝗠⟩
 
+
+/--
+  `WeakClassical` from Ariola (2007)
+-/
 protected abbrev WeakClassical : Hilbert α := ⟨𝗣𝗲⟩
 
+end systems
 
-end Hilbert
 
 
 namespace Deduction
 
-variable {Λ : Hilbert α}
-
 open System
 
-noncomputable def rec! {α : Type u} {Λ : Hilbert α}
-  {motive : (a : Formula α) → Λ ⊢! a → Sort u_1}
-  (eaxm   : ∀ {φ}, (a : φ ∈ Ax(Λ)) → motive φ ⟨eaxm a⟩)
-  (mdp    : ∀ {φ ψ}, {hpq : Λ ⊢! (φ ➝ ψ)} → {hp : Λ ⊢! φ} → motive (φ ➝ ψ) hpq → motive φ hp → motive ψ (hpq ⨀ hp))
+lemma eaxm! {H : Hilbert α} {φ : Formula α} (h : φ ∈ H.axioms) : H ⊢! φ := ⟨eaxm h⟩
+
+noncomputable def rec! {α : Type u} {H : Hilbert α}
+  {motive : (a : Formula α) → H ⊢! a → Sort u_1}
+  (eaxm   : ∀ {φ}, (a : φ ∈ H.axioms) → motive φ ⟨eaxm a⟩)
+  (mdp    : ∀ {φ ψ}, {hpq : H ⊢! (φ ➝ ψ)} → {hp : H ⊢! φ} → motive (φ ➝ ψ) hpq → motive φ hp → motive ψ (hpq ⨀ hp))
   (verum  : motive ⊤ verum!)
   (imply₁ : ∀ {φ ψ},   motive (φ ➝ ψ ➝ φ) imply₁!)
   (imply₂ : ∀ {φ ψ χ}, motive ((φ ➝ ψ ➝ χ) ➝ (φ ➝ ψ) ➝ φ ➝ χ) imply₂!)
@@ -138,7 +150,7 @@ noncomputable def rec! {α : Type u} {Λ : Hilbert α}
   (or₂    : ∀ {φ ψ},   motive (ψ ➝ φ ⋎ ψ) or₂!)
   (or₃    : ∀ {φ ψ χ}, motive ((φ ➝ χ) ➝ (ψ ➝ χ) ➝ φ ⋎ ψ ➝ χ) or₃!)
   (neg_equiv : ∀ {φ}, motive (Axioms.NegEquiv φ) neg_equiv!) :
-  {a : Formula α} → (t : Λ ⊢! a) → motive a t := by
+  {a : Formula α} → (t : H ⊢! a) → motive a t := by
   intro φ d;
   induction d.some with
   | eaxm h => exact eaxm h
@@ -150,10 +162,10 @@ end Deduction
 
 open System
 
-variable {Λ₁ Λ₂ : Hilbert α}
+section
 
-lemma weaker_than_of_subset_axiomset' (hMaxm : ∀ {φ : Formula α}, φ ∈ Ax(Λ₁) → Λ₂ ⊢! φ)
-  : Λ₁ ≤ₛ Λ₂ := by
+lemma weaker_than_of_subset_axiomset' {H₁ H₂ : Hilbert α} (hMaxm : ∀ {φ : Formula α}, φ ∈ H₁.axioms → H₂ ⊢! φ)
+  : H₁ ≤ₛ H₂ := by
   apply System.weakerThan_iff.mpr;
   intro φ h;
   induction h using Deduction.rec! with
@@ -161,30 +173,30 @@ lemma weaker_than_of_subset_axiomset' (hMaxm : ∀ {φ : Formula α}, φ ∈ Ax(
   | mdp ihpq ihp => exact ihpq ⨀ ihp;
   | _ => simp;
 
-lemma weaker_than_of_subset_axiomset (hSubset : Ax(Λ₁) ⊆ Ax(Λ₂) := by aesop) : Λ₁ ≤ₛ Λ₂ := by
+lemma weaker_than_of_subset_axiomset {H₁ H₂ : Hilbert α} (hSubset : H₁.axioms ⊆ H₂.axioms := by aesop) : H₁ ≤ₛ H₂ := by
   apply weaker_than_of_subset_axiomset';
   intro φ hp;
   apply eaxm! $ hSubset hp;
 
-lemma Int_weaker_than_Cl : (𝐈𝐧𝐭 : Hilbert α) ≤ₛ 𝐂𝐥 := weaker_than_of_subset_axiomset
+lemma Int_weaker_than_Cl : (Hilbert.Int α) ≤ₛ (Hilbert.Cl α) := weaker_than_of_subset_axiomset
 
-lemma Int_weaker_than_KC : (𝐈𝐧𝐭 : Hilbert α) ≤ₛ 𝐊𝐂 := weaker_than_of_subset_axiomset
+lemma Int_weaker_than_KC : (Hilbert.Int α) ≤ₛ (Hilbert.KC α) := weaker_than_of_subset_axiomset
 
-lemma Int_weaker_than_LC : (𝐈𝐧𝐭 : Hilbert α) ≤ₛ 𝐋𝐂 := weaker_than_of_subset_axiomset
+lemma Int_weaker_than_LC : (Hilbert.Int α) ≤ₛ (Hilbert.LC α) := weaker_than_of_subset_axiomset
 
-lemma KC_weaker_than_Cl : (𝐊𝐂 : Hilbert α) ≤ₛ 𝐂𝐥 := by
+lemma KC_weaker_than_Cl : (Hilbert.KC α) ≤ₛ (Hilbert.Cl α) := weaker_than_of_subset_axiomset' $ by
+  rintro φ (⟨_, rfl⟩ | ⟨_, rfl⟩) <;> simp;
+
+lemma LC_weaker_than_Cl [DecidableEq α] : (Hilbert.LC α) ≤ₛ (Hilbert.Cl α) := by
   apply weaker_than_of_subset_axiomset';
-  intro φ hp;
-  rcases hp with (⟨_, rfl⟩ | ⟨_, rfl⟩) <;> simp;
+  rintro φ (⟨_, rfl⟩ | ⟨_, _, rfl⟩) <;> simp;
 
-lemma LC_weaker_than_Cl [DecidableEq α] : (𝐋𝐂 : Hilbert α) ≤ₛ 𝐂𝐥 := by
-  apply weaker_than_of_subset_axiomset';
-  intro φ hp;
-  rcases hp with (⟨_, rfl⟩ | ⟨_, _, rfl⟩) <;> simp;
+end
 
-variable {φ : Formula α}
 
-theorem iff_provable_dn_efq_dne_provable [DecidableEq α] : 𝐈𝐧𝐭 ⊢! ∼∼φ ↔ 𝐂𝐥 ⊢! φ := by
+section Glivenko
+
+theorem iff_provable_dn_efq_dne_provable [DecidableEq α] : (Hilbert.Int α) ⊢! ∼∼φ ↔ (Hilbert.Cl α) ⊢! φ := by
   constructor;
   . intro d; exact dne'! $ Int_weaker_than_Cl d;
   . intro d;
@@ -199,7 +211,7 @@ theorem iff_provable_dn_efq_dne_provable [DecidableEq α] : 𝐈𝐧𝐭 ⊢! �
         subst hq;
         apply neg_equiv'!.mpr;
         apply FiniteContext.deduct'!;
-        have : [∼(ψ ⋎ ∼ψ)] ⊢[𝐈𝐧𝐭]! ∼ψ ⋏ ∼∼ψ := demorgan₃'! $ FiniteContext.id!;
+        have : [∼(ψ ⋎ ∼ψ)] ⊢[Hilbert.Int α]! ∼ψ ⋏ ∼∼ψ := demorgan₃'! $ FiniteContext.id!;
         exact neg_mdp! (and₂'! this) (and₁'! this);
     | @mdp φ ψ h₁ h₂ ih₁ ih₂ =>
       exact (dn_distribute_imply'! $ ih₁ ⟨h₁⟩) ⨀ ih₂ ⟨h₂⟩;
@@ -207,9 +219,14 @@ theorem iff_provable_dn_efq_dne_provable [DecidableEq α] : 𝐈𝐧𝐭 ⊢! �
 
 alias glivenko := iff_provable_dn_efq_dne_provable
 
-theorem iff_provable_neg_efq_provable_neg_efq [DecidableEq α] : 𝐈𝐧𝐭 ⊢! ∼φ ↔ 𝐂𝐥 ⊢! ∼φ := by
+theorem iff_provable_neg_efq_provable_neg_efq [DecidableEq α] : (Hilbert.Int α) ⊢! ∼φ ↔ (Hilbert.Cl α) ⊢! ∼φ := by
   constructor;
   . intro d; exact glivenko.mp $ dni'! d;
   . intro d; exact tne'! $ glivenko.mpr d;
+
+end Glivenko
+
+
+end Hilbert
 
 end LO.IntProp
