Foundation/Modal/Boxdot/Basic.lean
@@ -12,20 +12,21 @@ def Formula.BoxdotTranslation : Formula α → Formula α
 postfix:90 "ᵇ" => Formula.BoxdotTranslation
 
 
-class BoxdotProperty (Λ₁ Λ₂ : Hilbert α) where
-  bdp {φ} : Λ₁ ⊢! φ ↔ Λ₂ ⊢! φᵇ
+class BoxdotProperty (H₁ H₂ : Hilbert α) where
+  bdp {φ} : H₁ ⊢! φ ↔ H₂ ⊢! φᵇ
 
 
 open System
 open Formula
+open Hilbert.Deduction
 
 variable {φ : Formula α}
 
 theorem boxdotTranslated
-  {Λ₁ Λ₂ : Hilbert α} [Λ₁.IsNormal] [Λ₂.IsNormal]
-  (h : ∀ φ ∈ Λ₁.axioms, Λ₂ ⊢! φᵇ) : Λ₁ ⊢! φ → Λ₂ ⊢! φᵇ := by
+  {H₁ H₂ : Hilbert α} [H₁.IsNormal] [H₂.IsNormal]
+  (h : ∀ φ ∈ H₁.axioms, H₂ ⊢! φᵇ) : H₁ ⊢! φ → H₂ ⊢! φᵇ := by
   intro d;
-  induction d using Deduction.inducition_with_necOnly! with
+  induction d using inducition_with_necOnly! with
   | hMaxm hs => exact h _ hs;
   | hNec ihp =>
     dsimp [BoxdotTranslation];
@@ -37,7 +38,7 @@ theorem boxdotTranslated
     dsimp only [BoxdotTranslation];
     trivial;
 
-lemma boxdotTranslatedK4_of_S4 : 𝐒𝟒 ⊢! φ → 𝐊𝟒 ⊢! φᵇ := boxdotTranslated $ by
+lemma boxdotTranslatedK4_of_S4 : (Hilbert.S4 α) ⊢! φ → (Hilbert.K4 α) ⊢! φᵇ := boxdotTranslated $ by
   intro φ hp;
   simp at hp;
   rcases hp with (⟨_, _, rfl⟩ | ⟨_, rfl⟩ | ⟨_, rfl⟩);
@@ -45,19 +46,19 @@ lemma boxdotTranslatedK4_of_S4 : 𝐒𝟒 ⊢! φ → 𝐊𝟒 ⊢! φᵇ := box
   . dsimp [BoxdotTranslation]; exact boxdot_axiomT!;
   . dsimp [BoxdotTranslation]; exact boxdot_axiomFour!
 
-lemma iff_boxdotTranslation_S4 : 𝐒𝟒 ⊢! φ ⭤ φᵇ := by
+lemma iff_boxdotTranslation_S4 : (Hilbert.S4 α) ⊢! φ ⭤ φᵇ := by
   induction φ using Formula.rec' with
   | hbox φ ihp => exact iff_trans''! (box_iff! ihp) iff_box_boxdot!;
   | himp φ ψ ihp ihq => exact imp_replace_iff! ihp ihq;
   | _ => exact iff_id!;
 
-lemma S4_of_boxdotTranslatedK4 (h : 𝐊𝟒 ⊢! φᵇ) : 𝐒𝟒 ⊢! φ := by
-  exact (and₂'! iff_boxdotTranslation_S4) ⨀ (weakerThan_iff.mp $ K4_weakerThan_S4) h
+lemma S4_of_boxdotTranslatedK4 (h : (Hilbert.K4 α) ⊢! φᵇ) : (Hilbert.S4 α) ⊢! φ := by
+  exact (and₂'! iff_boxdotTranslation_S4) ⨀ (weakerThan_iff.mp $ Hilbert.K4_weakerThan_S4) h
 
-theorem iff_S4_boxdotTranslatedK4 : 𝐒𝟒 ⊢! φ ↔ 𝐊𝟒 ⊢! φᵇ := by
+theorem iff_S4_boxdotTranslatedK4 : (Hilbert.S4 α) ⊢! φ ↔ (Hilbert.K4 α) ⊢! φᵇ := by
   constructor;
   . apply boxdotTranslatedK4_of_S4;
   . apply S4_of_boxdotTranslatedK4;
-instance : BoxdotProperty (𝐒𝟒 : Hilbert α) 𝐊𝟒 := ⟨iff_S4_boxdotTranslatedK4⟩
+instance : BoxdotProperty (Hilbert.S4 α) (Hilbert.K4 α) := ⟨iff_S4_boxdotTranslatedK4⟩
 
 end LO.Modal
