Foundation/Modal/Hilbert.lean
@@ -6,10 +6,11 @@ namespace LO.Modal
 
 variable {α : Type*}
 
+
 section
 
 /-- instance of inference rule -/
-structure InferenceRule (α : Type*) where
+structure Hilbert.InferenceRule (α : Type*) where
   antecedents : List (Formula α)
   consequence : Formula α
   /--
@@ -18,6 +19,8 @@ structure InferenceRule (α : Type*) where
   so more than one antecedent is required.
   -/
   antecedents_nonempty : antecedents ≠ [] := by simp
+
+namespace Hilbert.InferenceRule
 
 abbrev Necessitation (φ : Formula α) : InferenceRule α := ⟨[φ], □φ, by simp⟩
 abbrev Necessitation.set : Set (InferenceRule α) := { Necessitation φ | φ }
@@ -31,103 +34,107 @@ abbrev HenkinRule (φ : Formula α) : InferenceRule α := ⟨[□φ ⭤ φ], φ,
 abbrev HenkinRule.set : Set (InferenceRule α) := { HenkinRule φ | φ }
 notation "⟮Henkin⟯" => HenkinRule.set
 
+end Hilbert.InferenceRule
+
 end
+
 
 structure Hilbert (α : Type*) where
   axioms : Theory α
-  rules : Set (InferenceRule α)
+  rules : Set (Hilbert.InferenceRule α)
 
-inductive Deduction (Λ : Hilbert α) : (Formula α) → Type _
-  | maxm {φ}     : φ ∈ Λ.axioms → Deduction Λ φ
-  | rule {rl}    : rl ∈ Λ.rules → (∀ {φ}, φ ∈ rl.antecedents → Deduction Λ φ) → Deduction Λ rl.consequence
-  | mdp {φ ψ}    : Deduction Λ (φ ➝ ψ) → Deduction Λ φ → Deduction Λ ψ
-  | imply₁ φ ψ   : Deduction Λ $ Axioms.Imply₁ φ ψ
-  | imply₂ φ ψ χ : Deduction Λ $ Axioms.Imply₂ φ ψ χ
-  | ec φ ψ       : Deduction Λ $ Axioms.ElimContra φ ψ
 
-namespace Deduction
+inductive Hilbert.Deduction (H : Hilbert α) : (Formula α) → Type _
+  | maxm {φ}     : φ ∈ H.axioms → Deduction H φ
+  | rule {rl}    : rl ∈ H.rules → (∀ {φ}, φ ∈ rl.antecedents → Deduction H φ) → Deduction H rl.consequence
+  | mdp {φ ψ}    : Deduction H (φ ➝ ψ) → Deduction H φ → Deduction H ψ
+  | imply₁ φ ψ   : Deduction H $ Axioms.Imply₁ φ ψ
+  | imply₂ φ ψ χ : Deduction H $ Axioms.Imply₂ φ ψ χ
+  | ec φ ψ       : Deduction H $ Axioms.ElimContra φ ψ
 
-variable {Λ Λ₁ Λ₂ : Hilbert α}
+namespace Hilbert.Deduction
+
+variable {H H₁ H₂ : Hilbert α}
 
 instance : System (Formula α) (Hilbert α) := ⟨Deduction⟩
 
-instance : System.Lukasiewicz Λ where
+instance : System.Lukasiewicz H where
   mdp := mdp
   imply₁ := imply₁
   imply₂ := imply₂
   elim_contra := ec
 
-instance : System.Classical Λ where
+instance : System.Classical H where
 
-instance : System.HasDiaDuality Λ := inferInstance
+instance : System.HasDiaDuality H := inferInstance
 
-lemma maxm! {φ} (h : φ ∈ Λ.axioms) : Λ ⊢! φ := ⟨maxm h⟩
+lemma maxm! {φ} (h : φ ∈ H.axioms) : H ⊢! φ := ⟨maxm h⟩
 
-end Deduction
+end Hilbert.Deduction
 
 
 namespace Hilbert
 
 open Deduction
 
-class HasNecessitation (Λ : Hilbert α) where
-  has_necessitation : ⟮Nec⟯ ⊆ Λ.rules := by aesop
+class HasNecessitation (H : Hilbert α) where
+  has_necessitation : ⟮Nec⟯ ⊆ H.rules := by aesop
 
-instance [HasNecessitation Λ] : System.Necessitation Λ where
-  nec := @λ φ d => rule (show { antecedents := [φ], consequence := □φ } ∈ Λ.rules by apply HasNecessitation.has_necessitation; simp_all) (by aesop);
-
-
-class HasLoebRule (Λ : Hilbert α) where
-  has_loeb : ⟮Loeb⟯ ⊆ Λ.rules := by aesop
-
-instance [HasLoebRule Λ] : System.LoebRule Λ where
-  loeb := @λ φ d => rule (show { antecedents := [□φ ➝ φ], consequence := φ } ∈ Λ.rules by apply HasLoebRule.has_loeb; simp_all) (by aesop);
+instance [HasNecessitation H] : System.Necessitation H where
+  nec := @λ φ d => rule (show { antecedents := [φ], consequence := □φ } ∈ H.rules by apply HasNecessitation.has_necessitation; simp_all) (by aesop);
 
 
-class HasHenkinRule (Λ : Hilbert α) where
-  has_henkin : ⟮Henkin⟯ ⊆ Λ.rules := by aesop
+class HasLoebRule (H : Hilbert α) where
+  has_loeb : ⟮Loeb⟯ ⊆ H.rules := by aesop
 
-instance [HasHenkinRule Λ] : System.HenkinRule Λ where
-  henkin := @λ φ d => rule (show { antecedents := [□φ ⭤ φ], consequence := φ } ∈ Λ.rules by apply HasHenkinRule.has_henkin; simp_all) (by aesop);
+instance [HasLoebRule H] : System.LoebRule H where
+  loeb := @λ φ d => rule (show { antecedents := [□φ ➝ φ], consequence := φ } ∈ H.rules by apply HasLoebRule.has_loeb; simp_all) (by aesop);
 
 
-class HasNecOnly (Λ : Hilbert α) where
-  has_necessitation_only : Λ.rules = ⟮Nec⟯ := by rfl
+class HasHenkinRule (H : Hilbert α) where
+  has_henkin : ⟮Henkin⟯ ⊆ H.rules := by aesop
 
-instance [h : HasNecOnly Λ] : Λ.HasNecessitation where
+instance [HasHenkinRule H] : System.HenkinRule H where
+  henkin := @λ φ d => rule (show { antecedents := [□φ ⭤ φ], consequence := φ } ∈ H.rules by apply HasHenkinRule.has_henkin; simp_all) (by aesop);
+
+
+class HasNecOnly (H : Hilbert α) where
+  has_necessitation_only : H.rules = ⟮Nec⟯ := by rfl
+
+instance [h : HasNecOnly H] : H.HasNecessitation where
   has_necessitation := by rw [h.has_necessitation_only]
 
-class HasAxiomK (Λ : Hilbert α) where
-  has_axiomK : 𝗞 ⊆ Λ.axioms := by aesop
+class HasAxiomK (H : Hilbert α) where
+  has_axiomK : 𝗞 ⊆ H.axioms := by aesop
 
-instance [HasAxiomK Λ] : System.HasAxiomK Λ where
+instance [HasAxiomK H] : System.HasAxiomK H where
   K _ _ := maxm (by apply HasAxiomK.has_axiomK; simp_all)
 
-class IsNormal (Λ : Hilbert α) extends Λ.HasNecOnly, Λ.HasAxiomK where
+class IsNormal (H : Hilbert α) extends H.HasNecOnly, H.HasAxiomK where
 
-instance [IsNormal Λ] : System.K Λ where
+instance {H : Hilbert α} [H.IsNormal] : System.K H where
 
 end Hilbert
 
 
-namespace Deduction
+namespace Hilbert.Deduction
 
 open Hilbert
 
-variable {Λ : Hilbert α}
+variable {H : Hilbert α}
 
 noncomputable def inducition!
-  {motive  : (φ : Formula α) → Λ ⊢! φ → Sort*}
-  (hRules  : (r : InferenceRule α) → (hr : r ∈ Λ.rules) →
-             (hant : ∀ {φ}, φ ∈ r.antecedents → Λ ⊢! φ) →
+  {motive  : (φ : Formula α) → H ⊢! φ → Sort*}
+  (hRules  : (r : InferenceRule α) → (hr : r ∈ H.rules) →
+             (hant : ∀ {φ}, φ ∈ r.antecedents → H ⊢! φ) →
              (ih : ∀ {φ}, (hp : φ ∈ r.antecedents) →
              motive φ (hant hp)) → motive r.consequence ⟨rule hr (λ hp => (hant hp).some)⟩)
-  (hMaxm     : ∀ {φ}, (h : φ ∈ Λ.axioms) → motive φ ⟨maxm h⟩)
-  (hMdp      : ∀ {φ ψ}, {hpq : Λ ⊢! φ ➝ ψ} → {hp : Λ ⊢! φ} → motive (φ ➝ ψ) hpq → motive φ hp → motive ψ ⟨mdp hpq.some hp.some⟩)
+  (hMaxm     : ∀ {φ}, (h : φ ∈ H.axioms) → motive φ ⟨maxm h⟩)
+  (hMdp      : ∀ {φ ψ}, {hpq : H ⊢! φ ➝ ψ} → {hp : H ⊢! φ} → motive (φ ➝ ψ) hpq → motive φ hp → motive ψ ⟨mdp hpq.some hp.some⟩)
   (hImply₁     : ∀ {φ ψ}, motive (φ ➝ ψ ➝ φ) $ ⟨imply₁ φ ψ⟩)
   (hImply₂     : ∀ {φ ψ χ}, motive ((φ ➝ ψ ➝ χ) ➝ (φ ➝ ψ) ➝ φ ➝ χ) $ ⟨imply₂ φ ψ χ⟩)
   (hElimContra : ∀ {φ ψ}, motive (Axioms.ElimContra φ ψ) $ ⟨ec φ ψ⟩)
-  : ∀ {φ}, (d : Λ ⊢! φ) → motive φ d := by
+  : ∀ {φ}, (d : H ⊢! φ) → motive φ d := by
   intro φ d;
   induction d.some with
   | maxm h => exact hMaxm h
@@ -138,15 +145,15 @@ noncomputable def inducition!
   | ec => exact hElimContra
 
 /-- Useful induction for normal modal logic. -/
-noncomputable def inducition_with_necOnly! [Λ.HasNecOnly]
-  {motive  : (φ : Formula α) → Λ ⊢! φ → Prop}
-  (hMaxm   : ∀ {φ}, (h : φ ∈ Λ.axioms) → motive φ ⟨maxm h⟩)
-  (hMdp    : ∀ {φ ψ}, {hpq : Λ ⊢! φ ➝ ψ} → {hp : Λ ⊢! φ} → motive (φ ➝ ψ) hpq → motive φ hp → motive ψ (hpq ⨀ hp))
-  (hNec    : ∀ {φ}, {hp : Λ ⊢! φ} → (ihp : motive φ hp) → motive (□φ) (System.nec! hp))
+noncomputable def inducition_with_necOnly! [H.HasNecOnly]
+  {motive  : (φ : Formula α) → H ⊢! φ → Prop}
+  (hMaxm   : ∀ {φ}, (h : φ ∈ H.axioms) → motive φ ⟨maxm h⟩)
+  (hMdp    : ∀ {φ ψ}, {hpq : H ⊢! φ ➝ ψ} → {hp : H ⊢! φ} → motive (φ ➝ ψ) hpq → motive φ hp → motive ψ (hpq ⨀ hp))
+  (hNec    : ∀ {φ}, {hp : H ⊢! φ} → (ihp : motive φ hp) → motive (□φ) (System.nec! hp))
   (hImply₁   : ∀ {φ ψ}, motive (φ ➝ ψ ➝ φ) $ ⟨imply₁ φ ψ⟩)
   (hImply₂   : ∀ {φ ψ χ}, motive ((φ ➝ ψ ➝ χ) ➝ (φ ➝ ψ) ➝ φ ➝ χ) $ ⟨imply₂ φ ψ χ⟩)
   (hElimContra : ∀ {φ ψ}, motive (Axioms.ElimContra φ ψ) $ ⟨ec φ ψ⟩)
-  : ∀ {φ}, (d : Λ ⊢! φ) → motive φ d := by
+  : ∀ {φ}, (d : H ⊢! φ) → motive φ d := by
   intro φ d;
   induction d using Deduction.inducition! with
   | hMaxm h => exact hMaxm h
@@ -170,177 +177,163 @@ macro_rules | `(tactic| trivial) => `(tactic|
   )
 macro_rules | `(tactic| trivial) => `(tactic | apply dne!)
 
-end Deduction
+end Hilbert.Deduction
 
 
-abbrev Hilbert.theorems (Λ : Hilbert α) := System.theory Λ
+namespace Hilbert
 
+abbrev theorems (H : Hilbert α) := System.theory H
+
+
+section K
+
+variable (α)
 
 protected abbrev K : Hilbert α := ⟨𝗞, ⟮Nec⟯⟩
-notation "𝐊" => Modal.K
-instance : 𝐊.IsNormal (α := α) where
+instance : (Hilbert.K α).IsNormal where
 
-abbrev ExtK (Ax : Theory α) : Hilbert α := ⟨𝗞 ∪ Ax, ⟮Nec⟯⟩
-prefix:max "𝜿" => ExtK
-instance : (𝜿Ax).IsNormal (α := α) where
-
-lemma K_is_extK_of_empty : (𝐊 : Hilbert α) = 𝜿∅ := by aesop;
-
-lemma K_is_extK_of_AxiomK : (𝐊 : Hilbert α) = 𝜿𝗞 := by aesop;
-
-namespace Normal
-
-open System
-
-variable {Ax : Theory α}
-
-lemma def_ax : (𝜿Ax).axioms = (𝗞 ∪ Ax) := by simp;
-
-lemma maxm! (h : φ ∈ Ax) : 𝜿Ax ⊢! φ := ⟨Deduction.maxm (by simp [def_ax]; right; assumption)⟩
-
-end Normal
+end K
 
 
--- tools of Modal Companion
-section
+section K_extension
 
-abbrev ExtS4 (Ax : Theory α) : Hilbert α := 𝜿(𝗧 ∪ 𝟰 ∪ Ax)
-prefix:max "𝝈" => ExtS4
-instance : System.S4 (𝝈Ax) where
+protected abbrev ExtK (Ax : Theory α) : Hilbert α := ⟨𝗞 ∪ Ax, ⟮Nec⟯⟩
+instance : (Hilbert.ExtK Ax).IsNormal where
+
+namespace ExtK
+
+lemma K_is_extK_of_empty : (Hilbert.K α) = (Hilbert.ExtK ∅) := by aesop;
+
+lemma K_is_extK_of_AxiomK : (Hilbert.K α) = (Hilbert.ExtK 𝗞) := by aesop;
+
+lemma def_ax : (Hilbert.ExtK Ax).axioms = (𝗞 ∪ Ax) := rfl
+
+lemma maxm! (h : φ ∈ Ax) : (Hilbert.ExtK Ax) ⊢! φ := ⟨Deduction.maxm (by simp [Hilbert.ExtK]; tauto)⟩
+
+end ExtK
+
+end K_extension
+
+
+section S4_extension
+
+protected abbrev ExtS4 (Ax : Theory α) : Hilbert α := Hilbert.ExtK (𝗧 ∪ 𝟰 ∪ Ax)
+instance : System.S4 (Hilbert.ExtS4 Ax) where
   T _ := Deduction.maxm $ Set.mem_of_subset_of_mem (by rfl) (by simp)
   Four _ := Deduction.maxm $ Set.mem_of_subset_of_mem (by rfl) (by simp)
 
-@[simp] lemma ExtS4.def_ax : (𝝈Ax).axioms = (𝗞 ∪ 𝗧 ∪ 𝟰 ∪ Ax) := by aesop;
+@[simp] lemma ExtS4.def_ax : (Hilbert.ExtS4 Ax).axioms = (𝗞 ∪ 𝗧 ∪ 𝟰 ∪ Ax) := by aesop;
 
-end
+end S4_extension
 
 
-protected abbrev KT : Hilbert α := 𝜿(𝗧)
-notation "𝐊𝐓" => Modal.KT
-instance : System.KT (𝐊𝐓 : Hilbert α) where
+section systems
+
+variable (α)
+
+protected abbrev KT : Hilbert α := Hilbert.ExtK $ 𝗧
+instance : System.KT (Hilbert.KT α) where
   T _ := Deduction.maxm $ Set.mem_of_subset_of_mem (by rfl) (by simp)
 
-protected abbrev KB : Hilbert α := 𝜿(𝗕)
-notation "𝐊𝐁" => Modal.KB
-instance : System.KB (𝐊𝐁 : Hilbert α) where
+protected abbrev KB : Hilbert α := Hilbert.ExtK $ 𝗕
+instance : System.KB (Hilbert.KB α) where
   B _ := Deduction.maxm $ Set.mem_of_subset_of_mem (by rfl) (by simp)
 
-protected abbrev KD : Hilbert α := 𝜿(𝗗)
-notation "𝐊𝐃" => Modal.KD
-instance : System.KD (𝐊𝐃 : Hilbert α) where
+protected abbrev KD : Hilbert α := Hilbert.ExtK $ 𝗗
+instance : System.KD (Hilbert.KD α) where
   D _ := Deduction.maxm $ Set.mem_of_subset_of_mem (by rfl) (by simp)
 
-protected abbrev KP : Hilbert α := 𝜿(𝗣)
-notation "𝐊𝐏" => Modal.KP
-instance : System.KP (𝐊𝐏 : Hilbert α) where
+protected abbrev KP : Hilbert α := Hilbert.ExtK $ 𝗣
+instance : System.KP (Hilbert.KP α) where
   P := Deduction.maxm $ Set.mem_of_subset_of_mem (by rfl) (by simp)
 
-protected abbrev KTB : Hilbert α := 𝜿(𝗧 ∪ 𝗕)
-notation "𝐊𝐓𝐁" => Modal.KTB
+protected abbrev KTB : Hilbert α := Hilbert.ExtK $ 𝗧 ∪ 𝗕
 
-protected abbrev K4 : Hilbert α := 𝜿(𝟰)
-notation "𝐊𝟒" => Modal.K4
-instance : System.K4 (𝐊𝟒 : Hilbert α) where
+protected abbrev K4 : Hilbert α := Hilbert.ExtK $ 𝟰
+instance : System.K4 (Hilbert.K4 α) where
   Four _ := Deduction.maxm $ Set.mem_of_subset_of_mem (by rfl) (by simp)
 
-protected abbrev K5 : Hilbert α := 𝜿(𝟱)
-notation "𝐊𝟓" => Modal.K5
-instance : System.K5 (𝐊𝟓 : Hilbert α) where
+protected abbrev K5 : Hilbert α := Hilbert.ExtK $ 𝟱
+instance : System.K5 (Hilbert.K5 α) where
   Five _ := Deduction.maxm $ Set.mem_of_subset_of_mem (by rfl) (by simp)
 
-protected abbrev S4 : Hilbert α := 𝝈(∅)
-notation "𝐒𝟒" => Modal.S4
-instance : System.S4 (𝐒𝟒 : Hilbert α) where
+protected abbrev S4 : Hilbert α := Hilbert.ExtS4 $ ∅
+instance : System.S4 (Hilbert.S4 α) where
   T _ := Deduction.maxm $ Set.mem_of_subset_of_mem (by rfl) (by simp)
   Four _ := Deduction.maxm $ Set.mem_of_subset_of_mem (by rfl) (by simp)
 
-protected abbrev S4Dot2 : Hilbert α := 𝝈(.𝟮)
-notation "𝐒𝟒.𝟐" => Modal.S4Dot2
+protected abbrev S4Dot2 : Hilbert α := Hilbert.ExtS4 $ .𝟮
 
-protected abbrev S4Dot3 : Hilbert α := 𝝈(.𝟯)
-notation "𝐒𝟒.𝟑" => Modal.S4Dot3
+protected abbrev S4Dot3 : Hilbert α := Hilbert.ExtS4 $ .𝟯
 
-protected abbrev S4Grz : Hilbert α := 𝝈(𝗚𝗿𝘇) -- S4 + 𝗚𝗿𝘇
-notation "𝐒𝟒𝐆𝐫𝐳" => Modal.S4Grz
+protected abbrev S4Grz : Hilbert α := Hilbert.ExtS4 $ 𝗚𝗿𝘇
 
-protected abbrev KT4B : Hilbert α := 𝝈(𝗕)
-notation "𝐊𝐓𝟒𝐁" => Modal.KT4B
+protected abbrev KT4B : Hilbert α := Hilbert.ExtS4 $ 𝗕
 
-protected abbrev S5 : Hilbert α := 𝜿(𝗧 ∪ 𝟱)
-notation "𝐒𝟓" => Modal.S5
-instance : System.S5 (𝐒𝟓 : Hilbert α) where
+protected abbrev S5 : Hilbert α := Hilbert.ExtK $ 𝗧 ∪ 𝟱
+instance : System.S5 (Hilbert.S5 α) where
   T _ := Deduction.maxm $ Set.mem_of_subset_of_mem (by rfl) (by simp)
   Five _ := Deduction.maxm $ Set.mem_of_subset_of_mem (by rfl) (by simp)
 
-protected abbrev S5Grz : Hilbert α := 𝜿(𝗧 ∪ 𝟱 ∪ 𝗚𝗿𝘇) -- 𝐒𝟓 + 𝗚𝗿𝘇
-notation "𝐒𝟓𝐆𝐫𝐳" => Modal.S5Grz
-instance : System.S5Grz (𝐒𝟓𝐆𝐫𝐳 : Hilbert α) where
+protected abbrev S5Grz : Hilbert α := Hilbert.ExtK $ 𝗧 ∪ 𝟱 ∪ 𝗚𝗿𝘇
+instance : System.S5Grz (Hilbert.S5Grz α) where
   T _ := Deduction.maxm $ Set.mem_of_subset_of_mem (by rfl) (by simp)
   Five _ := Deduction.maxm $ Set.mem_of_subset_of_mem (by rfl) (by simp)
   Grz _ := Deduction.maxm $ Set.mem_of_subset_of_mem (by rfl) (by simp)
 
-protected abbrev Triv : Hilbert α := 𝜿(𝗧 ∪ 𝗧𝗰)
-notation "𝐓𝐫𝐢𝐯" => Modal.Triv
-instance : System.Triv (𝐓𝐫𝐢𝐯 : Hilbert α) where
+protected abbrev Triv : Hilbert α := Hilbert.ExtK $ 𝗧 ∪ 𝗧𝗰
+instance : System.Triv (Hilbert.Triv α) where
   T _ := Deduction.maxm $ Set.mem_of_subset_of_mem (by rfl) (by simp)
   Tc _ := Deduction.maxm $ Set.mem_of_subset_of_mem (by rfl) (by simp)
 
-protected abbrev Ver : Hilbert α := 𝜿(𝗩𝗲𝗿)
-notation "𝐕𝐞𝐫" => Modal.Ver
-instance : System.Ver (𝐕𝐞𝐫 : Hilbert α) where
+protected abbrev Ver : Hilbert α := Hilbert.ExtK $ 𝗩𝗲𝗿
+instance : System.Ver (Hilbert.Ver α) where
   Ver _ := Deduction.maxm $ Set.mem_of_subset_of_mem (by rfl) (by simp)
 
-protected abbrev GL : Hilbert α := 𝜿(𝗟)
-notation "𝐆𝐋" => Modal.GL
-instance : System.GL (𝐆𝐋 : Hilbert α) where
+protected abbrev GL : Hilbert α := Hilbert.ExtK $ 𝗟
+instance : System.GL (Hilbert.GL α) where
   L _ := Deduction.maxm $ Set.mem_of_subset_of_mem (by rfl) (by simp)
 
-protected abbrev Grz : Hilbert α := 𝜿(𝗚𝗿𝘇)
-notation "𝐆𝐫𝐳" => Modal.Grz
-instance : System.Grz (𝐆𝐫𝐳 : Hilbert α) where
+protected abbrev Grz : Hilbert α := Hilbert.ExtK $ 𝗚𝗿𝘇
+instance : System.Grz (Hilbert.Grz α) where
   Grz _ := Deduction.maxm $ Set.mem_of_subset_of_mem (by rfl) (by simp)
 
-protected abbrev K4H : Hilbert α := 𝜿(𝟰 ∪ 𝗛)
-notation "𝐊𝟒𝐇" => Modal.K4H
-instance : System.K4H (𝐊𝟒𝐇 : Hilbert α) where
+protected abbrev K4H : Hilbert α := Hilbert.ExtK $ 𝟰 ∪ 𝗛
+instance : System.K4H (Hilbert.K4H α) where
   Four _ := Deduction.maxm $ Set.mem_of_subset_of_mem (by rfl) (by simp)
   H _ := Deduction.maxm $ Set.mem_of_subset_of_mem (by rfl) (by simp)
 
--- Non-normal modal logic
-
 protected abbrev K4Loeb : Hilbert α := ⟨𝗞 ∪ 𝟰, ⟮Nec⟯ ∪ ⟮Loeb⟯⟩
-notation "𝐊𝟒(𝐋)" => Modal.K4Loeb
-instance : 𝐊𝟒(𝐋).HasAxiomK (α := α) where
-instance : 𝐊𝟒(𝐋).HasNecessitation (α := α) where
-instance : 𝐊𝟒(𝐋).HasLoebRule (α := α) where
-instance : System.K4Loeb (𝐊𝟒(𝐋) : Hilbert α) where
+instance : (Hilbert.K4Loeb α).HasAxiomK where
+instance : (Hilbert.K4Loeb α).HasNecessitation where
+instance : (Hilbert.K4Loeb α).HasLoebRule where
+instance : System.K4Loeb (Hilbert.K4Loeb α) where
   Four _ := Deduction.maxm $ Set.mem_of_subset_of_mem (by rfl) (by simp)
 
 protected abbrev K4Henkin : Hilbert α := ⟨𝗞 ∪ 𝟰, ⟮Nec⟯ ∪ ⟮Henkin⟯⟩
-notation "𝐊𝟒(𝐇)" => Modal.K4Henkin
-instance : 𝐊𝟒(𝐇).HasAxiomK (α := α)  where
-instance : 𝐊𝟒(𝐇).HasNecessitation (α := α) where
-instance : 𝐊𝟒(𝐇).HasHenkinRule (α := α) where
-instance : System.K4Henkin (𝐊𝟒(𝐇) : Hilbert α) where
+instance : (Hilbert.K4Henkin α).HasAxiomK  where
+instance : (Hilbert.K4Henkin α).HasNecessitation where
+instance : (Hilbert.K4Henkin α).HasHenkinRule where
+instance : System.K4Henkin (Hilbert.K4Henkin α) where
   Four _ := Deduction.maxm $ Set.mem_of_subset_of_mem (by rfl) (by simp)
 
 /--
   Solovey's Provability Logic of True Arithmetic.
   Remark necessitation is *not* permitted.
 -/
-protected abbrev GLS : Hilbert α := ⟨𝐆𝐋.theorems ∪ 𝗧, ∅⟩
-notation "𝐆𝐋𝐒" => Modal.GLS
-instance : System.HasAxiomK (𝐆𝐋𝐒 : Hilbert α) where
+protected abbrev GLS : Hilbert α := ⟨(Hilbert.GL α).theorems ∪ 𝗧, ∅⟩
+instance : System.HasAxiomK (Hilbert.GLS α) where
   K _ _ := Deduction.maxm $ Set.mem_of_subset_of_mem (by rfl) $ by simp [Hilbert.theorems, System.theory, System.axiomK!];
-instance : System.HasAxiomL (𝐆𝐋𝐒 : Hilbert α) where
+instance : System.HasAxiomL (Hilbert.GLS α) where
   L _ := Deduction.maxm $ Set.mem_of_subset_of_mem (by rfl) $ by simp [Hilbert.theorems, System.theory, System.axiomK!];
-instance : System.HasAxiomT (𝐆𝐋𝐒 : Hilbert α) where
+instance : System.HasAxiomT (Hilbert.GLS α) where
   T _ := Deduction.maxm $ Set.mem_of_subset_of_mem (by rfl) (by simp)
 
 /-- Logic of Pure Necessitation -/
 protected abbrev N : Hilbert α := ⟨∅, ⟮Nec⟯⟩
-notation "𝐍" => Modal.N
-instance : 𝐍.HasNecOnly (α := α) where
+instance : (Hilbert.N α).HasNecOnly where
+
+end systems
 
 
 section
@@ -349,9 +342,9 @@ variable [DecidableEq α]
 open System
 open Formula (atom)
 
-lemma normal_weakerThan_of_maxm {Λ₁ Λ₂ : Hilbert α} [Λ₁.IsNormal] [Λ₂.IsNormal]
-  (hMaxm : ∀ {φ : Formula α}, φ ∈ Λ₁.axioms → Λ₂ ⊢! φ)
-  : Λ₁ ≤ₛ Λ₂ := by
+lemma normal_weakerThan_of_maxm {H₁ H₂ : Hilbert α} [H₁.IsNormal] [H₂.IsNormal]
+  (hMaxm : ∀ {φ : Formula α}, φ ∈ H₁.axioms → H₂ ⊢! φ)
+  : H₁ ≤ₛ H₂ := by
   apply System.weakerThan_iff.mpr;
   intro φ h;
   induction h using Deduction.inducition_with_necOnly! with
@@ -360,77 +353,56 @@ lemma normal_weakerThan_of_maxm {Λ₁ Λ₂ : Hilbert α} [Λ₁.IsNormal] [Λ�
   | hNec ihp => exact nec! ihp;
   | _ => trivial;
 
-lemma normal_weakerThan_of_subset {Λ₁ Λ₂ : Hilbert α} [Λ₁.IsNormal] [Λ₂.IsNormal] (hSubset : Λ₁.axioms ⊆ Λ₂.axioms)
-  : Λ₁ ≤ₛ Λ₂ := by
+lemma normal_weakerThan_of_subset {H₁ H₂ : Hilbert α} [H₁.IsNormal] [H₂.IsNormal] (hSubset : H₁.axioms ⊆ H₂.axioms)
+  : H₁ ≤ₛ H₂ := by
   apply normal_weakerThan_of_maxm;
   intro φ hp;
   exact ⟨Deduction.maxm $ hSubset hp⟩;
 
-lemma K_weakerThan_KD : (𝐊 : Hilbert α) ≤ₛ 𝐊𝐃 := normal_weakerThan_of_subset $ by aesop;
 
-lemma K_weakerThan_KB : (𝐊 : Hilbert α) ≤ₛ 𝐊𝐁 := normal_weakerThan_of_subset $ by aesop;
+lemma K_weakerThan_KD : (Hilbert.K α) ≤ₛ (Hilbert.KD α) := normal_weakerThan_of_subset $ by aesop;
 
-lemma K_weakerThan_KT : (𝐊 : Hilbert α) ≤ₛ 𝐊𝐓 := normal_weakerThan_of_subset $ by aesop;
+lemma K_weakerThan_KB : (Hilbert.K α) ≤ₛ (Hilbert.KB α) := normal_weakerThan_of_subset $ by aesop;
 
-lemma K_weakerThan_K4 : (𝐊 : Hilbert α) ≤ₛ 𝐊𝟒 := normal_weakerThan_of_subset $ by aesop;
+lemma K_weakerThan_KT : (Hilbert.K α) ≤ₛ (Hilbert.KT α) := normal_weakerThan_of_subset $ by aesop;
 
-lemma K_weakerThan_K5 : (𝐊 : Hilbert α) ≤ₛ 𝐊𝟓 := normal_weakerThan_of_subset $ by aesop;
+lemma K_weakerThan_K4 : (Hilbert.K α) ≤ₛ (Hilbert.K4 α) := normal_weakerThan_of_subset $ by aesop;
 
-lemma KT_weakerThan_S4 : (𝐊𝐓 : Hilbert α) ≤ₛ 𝐒𝟒 := normal_weakerThan_of_subset $ by intro; aesop;
+lemma K_weakerThan_K5 : (Hilbert.K α) ≤ₛ (Hilbert.K5 α) := normal_weakerThan_of_subset $ by aesop;
 
-lemma K4_weakerThan_S4 : (𝐊𝟒 : Hilbert α) ≤ₛ 𝐒𝟒 := normal_weakerThan_of_subset $ by intro; aesop;
+lemma KT_weakerThan_S4 : (Hilbert.KT α) ≤ₛ (Hilbert.S4 α) := normal_weakerThan_of_subset $ by intro; aesop;
 
-lemma S4_weakerThan_S4Dot2 : (𝐒𝟒 : Hilbert α) ≤ₛ 𝐒𝟒.𝟐 := normal_weakerThan_of_subset $ by intro; aesop;
+lemma K4_weakerThan_S4 : (Hilbert.K4 α) ≤ₛ (Hilbert.S4 α) := normal_weakerThan_of_subset $ by intro; aesop;
 
-lemma S4_weakerThan_S4Dot3 : (𝐒𝟒 : Hilbert α) ≤ₛ 𝐒𝟒.𝟑 := normal_weakerThan_of_subset $ by intro; aesop;
+lemma S4_weakerThan_S4Dot2 : (Hilbert.S4 α) ≤ₛ (Hilbert.S4Dot2 α) := normal_weakerThan_of_subset $ by intro; aesop;
 
-lemma S4_weakerThan_S4Grz : (𝐒𝟒 : Hilbert α) ≤ₛ 𝐒𝟒𝐆𝐫𝐳 := normal_weakerThan_of_subset $ by intro; aesop;
+lemma S4_weakerThan_S4Dot3 : (Hilbert.S4 α) ≤ₛ (Hilbert.S4Dot3 α) := normal_weakerThan_of_subset $ by intro; aesop;
 
-lemma K_weakerThan_GL : (𝐊 : Hilbert α) ≤ₛ 𝐆𝐋 := normal_weakerThan_of_subset $ by intro; aesop;
+lemma S4_weakerThan_S4Grz : (Hilbert.S4 α) ≤ₛ (Hilbert.S4Grz α) := normal_weakerThan_of_subset $ by intro; aesop;
 
-lemma K4_weakerThan_Triv : (𝐊𝟒 : Hilbert α) ≤ₛ 𝐓𝐫𝐢𝐯 := by
-  apply normal_weakerThan_of_maxm;
-  intro φ hp;
-  rcases hp with (hK | hFour)
-  . obtain ⟨_, _, rfl⟩ := hK; exact axiomK!;
-  . obtain ⟨_, _, rfl⟩ := hFour; exact axiomFour!;
+lemma K_weakerThan_GL : (Hilbert.K α) ≤ₛ (Hilbert.GL α) := normal_weakerThan_of_subset $ by intro; aesop;
 
-lemma K4_weakerThan_GL : (𝐊𝟒 : Hilbert α) ≤ₛ 𝐆𝐋 := by
-  apply normal_weakerThan_of_maxm;
-  intro φ hp;
-  rcases hp with (hK | hFour)
-  . obtain ⟨_, _, rfl⟩ := hK; exact axiomK!;
-  . obtain ⟨_, _, rfl⟩ := hFour; exact axiomFour!;
+lemma K4_weakerThan_Triv : (Hilbert.K4 α) ≤ₛ (Hilbert.Triv α) := normal_weakerThan_of_maxm $ by
+  rintro φ (⟨_, _, rfl⟩ | ⟨_, _, rfl⟩) <;> simp;
 
-lemma KT_weakerThan_Grz : (𝐊𝐓 : Hilbert α) ≤ₛ 𝐆𝐫𝐳 := by
-  apply normal_weakerThan_of_maxm;
-  intro φ hp;
-  rcases hp with (hK | hGrz)
-  . obtain ⟨_, _, rfl⟩ := hK; exact axiomK!;
-  . obtain ⟨_, _, rfl⟩ := hGrz; exact axiomT!;
+lemma K4_weakerThan_GL : (Hilbert.K4 α) ≤ₛ (Hilbert.GL α) := normal_weakerThan_of_maxm $ by
+  rintro _ (⟨_, _, rfl⟩ | ⟨_, _, rfl⟩) <;> simp;
 
-lemma K4_weakerThan_Grz : (𝐊𝟒 : Hilbert α) ≤ₛ 𝐆𝐫𝐳 := by
-  apply normal_weakerThan_of_maxm;
-  intro φ hp;
-  rcases hp with (hK | hGrz)
-  . obtain ⟨_, _, rfl⟩ := hK; exact axiomK!;
-  . obtain ⟨_, _, rfl⟩ := hGrz; exact axiomFour!;
+lemma KT_weakerThan_Grz : (Hilbert.KT α) ≤ₛ (Hilbert.Grz α) := normal_weakerThan_of_maxm $ by
+  rintro _ (⟨_, _, rfl⟩ | ⟨_, _, rfl⟩) <;> simp;
 
+lemma K4_weakerThan_Grz : (Hilbert.K4 α) ≤ₛ (Hilbert.Grz α) := normal_weakerThan_of_maxm $ by
+  rintro _ (⟨_, _, rfl⟩ | ⟨_, _, rfl⟩) <;> simp;
 
-lemma KD_weakerThan_KP : (𝐊𝐃 : Hilbert α) ≤ₛ 𝐊𝐏 := normal_weakerThan_of_maxm $ by
-  rintro φ (⟨φ, ψ, rfl⟩ | ⟨φ, rfl⟩);
-  . exact axiomK!;
-  . exact axiomD!;
+lemma KD_weakerThan_KP : (Hilbert.KD α) ≤ₛ (Hilbert.KP α) := normal_weakerThan_of_maxm $ by
+  rintro _ (⟨_, _, rfl⟩ | ⟨_, rfl⟩) <;> simp;
 
-lemma KP_weakerThan_KD : (𝐊𝐏 : Hilbert α) ≤ₛ 𝐊𝐃 := normal_weakerThan_of_maxm $ by
-  rintro φ (⟨φ, ψ, rfl⟩ | ⟨_, rfl⟩);
-  . exact axiomK!;
-  . exact axiomP!;
+lemma KP_weakerThan_KD : (Hilbert.KP α) ≤ₛ (Hilbert.KD α) := normal_weakerThan_of_maxm $ by
+  rintro _ (⟨_, _, rfl⟩ | ⟨_, rfl⟩) <;> simp;
 
-lemma KD_equiv_KP : (𝐊𝐃 : Hilbert α) =ₛ 𝐊𝐏 := Equiv.antisymm_iff.mpr ⟨KD_weakerThan_KP, KP_weakerThan_KD⟩
+lemma KD_equiv_KP : (Hilbert.KD α) =ₛ (Hilbert.KP α) := Equiv.antisymm_iff.mpr ⟨KD_weakerThan_KP, KP_weakerThan_KD⟩
 
-
-lemma GL_weakerThan_K4Loeb : (𝐆𝐋 : Hilbert α) ≤ₛ 𝐊𝟒(𝐋) := by
+lemma GL_weakerThan_K4Loeb : (Hilbert.GL α) ≤ₛ (Hilbert.K4Loeb α) := by
   apply System.weakerThan_iff.mpr;
   intro φ h;
   induction h using Deduction.inducition_with_necOnly! with
@@ -442,7 +414,7 @@ lemma GL_weakerThan_K4Loeb : (𝐆𝐋 : Hilbert α) ≤ₛ 𝐊𝟒(𝐋) := by
   | hNec ihp => exact nec! ihp;
   | _ => trivial;
 
-lemma K4Loeb_weakerThan_K4Henkin : (𝐊𝟒(𝐋) : Hilbert α) ≤ₛ 𝐊𝟒(𝐇) := by
+lemma K4Loeb_weakerThan_K4Henkin : (Hilbert.K4Loeb α) ≤ₛ (Hilbert.K4Henkin α) := by
   apply System.weakerThan_iff.mpr;
   intro φ h;
   induction h using Deduction.inducition! with
@@ -457,7 +429,7 @@ lemma K4Loeb_weakerThan_K4Henkin : (𝐊𝟒(𝐋) : Hilbert α) ≤ₛ 𝐊𝟒
     . obtain ⟨φ, rfl⟩ := hLoeb; exact loeb! $ ihp $ by simp_all only [List.mem_singleton, forall_eq];
   | _ => trivial;
 
-lemma K4Henkin_weakerThan_K4H : (𝐊𝟒(𝐇) : Hilbert α) ≤ₛ 𝐊𝟒𝐇 := by
+lemma K4Henkin_weakerThan_K4H : (Hilbert.K4Henkin α) ≤ₛ (Hilbert.K4H α) := by
   apply System.weakerThan_iff.mpr;
   intro φ h;
   induction h using Deduction.inducition! with
@@ -472,7 +444,7 @@ lemma K4Henkin_weakerThan_K4H : (𝐊𝟒(𝐇) : Hilbert α) ≤ₛ 𝐊𝟒�
     . obtain ⟨φ, rfl⟩ := hHenkin; exact henkin! $ ihp $ by simp_all only [List.mem_singleton, forall_eq];
   | _ => trivial;
 
-lemma K4Henkin_weakerThan_GL : (𝐊𝟒𝐇 : Hilbert α) ≤ₛ 𝐆𝐋 := by
+lemma K4Henkin_weakerThan_GL : (Hilbert.K4H α) ≤ₛ (Hilbert.GL α) := by
   apply normal_weakerThan_of_maxm;
   intro φ hp;
   rcases hp with hK | hFour | hH
@@ -480,38 +452,30 @@ lemma K4Henkin_weakerThan_GL : (𝐊𝟒𝐇 : Hilbert α) ≤ₛ 𝐆𝐋 := by
   . obtain ⟨_, _, rfl⟩ := hFour; exact axiomFour!;
   . obtain ⟨_, _, rfl⟩ := hH; exact axiomH!;
 
-lemma GL_equiv_K4Loeb : (𝐆𝐋 : Hilbert α) =ₛ 𝐊𝟒(𝐋) := by
+lemma GL_equiv_K4Loeb : (Hilbert.GL α) =ₛ (Hilbert.K4Loeb α) := by
   apply Equiv.antisymm_iff.mpr;
   constructor;
   . exact GL_weakerThan_K4Loeb;
   . exact WeakerThan.trans (K4Loeb_weakerThan_K4Henkin) $ WeakerThan.trans K4Henkin_weakerThan_K4H K4Henkin_weakerThan_GL
 
-set_option linter.unusedSectionVars false in -- TODO: remove
-lemma GL_weakerThan_GLS : (𝐆𝐋 : Hilbert α) ≤ₛ 𝐆𝐋𝐒 := by
+omit [DecidableEq α] in
+lemma GL_weakerThan_GLS : (Hilbert.GL α) ≤ₛ (Hilbert.GLS α) := by
   apply System.weakerThan_iff.mpr;
   intro φ h;
   exact Deduction.maxm! (by left; simpa);
 
-lemma S5Grz_weakerThan_Triv : (𝐒𝟓𝐆𝐫𝐳 : Hilbert α) ≤ₛ 𝐓𝐫𝐢𝐯 := by
-  apply normal_weakerThan_of_maxm;
-  intro φ hp;
-  rcases hp with ⟨_, _, rfl⟩ | (⟨_, rfl⟩ | ⟨_, rfl⟩) | ⟨_, rfl⟩
-  . exact axiomK!;
-  . exact axiomT!;
-  . exact axiomFive!;
-  . exact axiomGrz!;
+lemma S5Grz_weakerThan_Triv : (Hilbert.S5Grz α) ≤ₛ (Hilbert.Triv α) := normal_weakerThan_of_maxm $ by
+  rintro φ (⟨_, _, rfl⟩ | (⟨_, rfl⟩ | ⟨_, rfl⟩) | ⟨_, rfl⟩) <;> simp;
 
-lemma Triv_weakerThan_S5Grz : (𝐓𝐫𝐢𝐯 : Hilbert α) ≤ₛ 𝐒𝟓𝐆𝐫𝐳 := by
-  apply normal_weakerThan_of_maxm;
-  intro φ hp;
-  rcases hp with ⟨_, _, rfl⟩ | ⟨_, rfl⟩ | ⟨_, rfl⟩
-  . exact axiomK!;
-  . exact axiomT!;
-  . exact axiomTc!;
+lemma Triv_weakerThan_S5Grz : (Hilbert.Triv α) ≤ₛ (Hilbert.S5Grz α) := normal_weakerThan_of_maxm $ by
+  rintro φ (⟨_, _, rfl⟩ | ⟨_, rfl⟩ | ⟨_, rfl⟩) <;> simp;
 
-lemma S5Grz_equiv_Triv : (𝐒𝟓𝐆𝐫𝐳 : Hilbert α) =ₛ 𝐓𝐫𝐢𝐯
+lemma S5Grz_equiv_Triv : (Hilbert.S5Grz α) =ₛ (Hilbert.Triv α)
   := Equiv.antisymm_iff.mpr ⟨S5Grz_weakerThan_Triv, Triv_weakerThan_S5Grz⟩
 
 end
+
+
+end Hilbert
 
 end LO.Modal
