Foundation/Modal/ModalCompanion/Basic.lean
@@ -20,14 +20,14 @@ def GoedelTranslation : IntProp.Formula α → Modal.Formula α
   | φ ➝ ψ => □((GoedelTranslation φ) ➝ (GoedelTranslation ψ))
 postfix:90 "ᵍ" => GoedelTranslation
 
-class ModalCompanion (iΛ : IntProp.Hilbert α) (mΛ : Modal.Hilbert α) where
-  companion : ∀ {φ : IntProp.Formula α}, iΛ ⊢! φ ↔ mΛ ⊢! φᵍ
+class ModalCompanion (iH : IntProp.Hilbert α) (mH : Modal.Hilbert α) where
+  companion : ∀ {φ : IntProp.Formula α}, iH ⊢! φ ↔ mH ⊢! φᵍ
 
 variable {α : Type u}
-variable {iΛ : IntProp.Hilbert α} {mΛ : Hilbert α}
+variable {iH : IntProp.Hilbert α} {mH : Hilbert α}
 variable {φ ψ χ : IntProp.Formula α}
 
-lemma axiomTc_GTranslate! [DecidableEq α] [System.K4 mΛ] : mΛ ⊢! φᵍ ➝ □φᵍ := by
+lemma axiomTc_GTranslate! [DecidableEq α] [System.K4 mH] : mH ⊢! φᵍ ➝ □φᵍ := by
   induction φ using IntProp.Formula.rec' with
   | hverum => exact imply₁'! (nec! verum!);
   | hfalsum => simp only [GoedelTranslation, efq!];
@@ -42,38 +42,38 @@ lemma axiomTc_GTranslate! [DecidableEq α] [System.K4 mΛ] : mΛ ⊢! φᵍ ➝ 
 
 section
 
-private lemma provable_efq_of_provable_S4.case_imply₁ [DecidableEq α] [System.K4 mΛ] : mΛ ⊢! (φ ➝ ψ ➝ φ)ᵍ := by
+private lemma provable_efq_of_provable_S4.case_imply₁ [DecidableEq α] [System.K4 mH] : mH ⊢! (φ ➝ ψ ➝ φ)ᵍ := by
   simp only [GoedelTranslation];
   exact nec! $ imp_trans''! axiomTc_GTranslate! $ axiomK'! $ nec! $ imply₁!;
 
-private lemma provable_efq_of_provable_S4.case_imply₂ [DecidableEq α] [System.S4 mΛ] : mΛ ⊢! ((φ ➝ ψ ➝ χ) ➝ (φ ➝ ψ) ➝ φ ➝ χ)ᵍ := by
+private lemma provable_efq_of_provable_S4.case_imply₂ [DecidableEq α] [System.S4 mH] : mH ⊢! ((φ ➝ ψ ➝ χ) ➝ (φ ➝ ψ) ➝ φ ➝ χ)ᵍ := by
   simp only [GoedelTranslation];
   apply nec! $ imp_trans''! (imp_trans''! (axiomK'! $ nec! ?b) axiomFour!) $ axiomK'! $ nec! $ imp_trans''! (axiomK'! $ nec! imply₂!) axiomK!;
   apply provable_iff_provable.mpr;
   apply deduct_iff.mpr;
   apply deduct_iff.mpr;
-  have : [φᵍ, φᵍ ➝ □(ψᵍ ➝ χᵍ)] ⊢[mΛ]! φᵍ := by_axm!;
-  have : [φᵍ, φᵍ ➝ □(ψᵍ ➝ χᵍ)] ⊢[mΛ]! (φᵍ ➝ □(ψᵍ ➝ χᵍ)) := by_axm!;
-  have : [φᵍ, φᵍ ➝ □(ψᵍ ➝ χᵍ)] ⊢[mΛ]! □(ψᵍ ➝ χᵍ) := (by assumption) ⨀ (by assumption);
+  have : [φᵍ, φᵍ ➝ □(ψᵍ ➝ χᵍ)] ⊢[mH]! φᵍ := by_axm!;
+  have : [φᵍ, φᵍ ➝ □(ψᵍ ➝ χᵍ)] ⊢[mH]! (φᵍ ➝ □(ψᵍ ➝ χᵍ)) := by_axm!;
+  have : [φᵍ, φᵍ ➝ □(ψᵍ ➝ χᵍ)] ⊢[mH]! □(ψᵍ ➝ χᵍ) := (by assumption) ⨀ (by assumption);
   exact axiomT'! this;
-private lemma provable_efq_of_provable_S4.case_and₃ [DecidableEq α] [System.K4 mΛ] : mΛ ⊢! (φ ➝ ψ ➝ φ ⋏ ψ)ᵍ := by
+private lemma provable_efq_of_provable_S4.case_and₃ [DecidableEq α] [System.K4 mH] : mH ⊢! (φ ➝ ψ ➝ φ ⋏ ψ)ᵍ := by
   simp only [GoedelTranslation];
   exact nec! $ imp_trans''! axiomTc_GTranslate! $ axiomK'! $ nec! $ and₃!
 
-private lemma provable_efq_of_provable_S4.case_or₃ [System.K4 mΛ] : mΛ ⊢! (((φ ➝ χ) ➝ (ψ ➝ χ) ➝ (φ ⋎ ψ ➝ χ)))ᵍ := by
+private lemma provable_efq_of_provable_S4.case_or₃ [System.K4 mH] : mH ⊢! (((φ ➝ χ) ➝ (ψ ➝ χ) ➝ (φ ⋎ ψ ➝ χ)))ᵍ := by
   simp only [GoedelTranslation];
   exact nec! $ imp_trans''! axiomFour! $ axiomK'! $ nec! $ imp_trans''! (axiomK'! $ nec! $ or₃!) axiomK!;
 
-private lemma provable_efq_of_provable_S4.case_neg_equiv [System.K4 mΛ] : mΛ ⊢! (Axioms.NegEquiv φ)ᵍ := by
+private lemma provable_efq_of_provable_S4.case_neg_equiv [System.K4 mH] : mH ⊢! (Axioms.NegEquiv φ)ᵍ := by
   simp only [GoedelTranslation];
   apply and₃'!;
   . exact nec! $ axiomK'! $ nec! $ and₁'! neg_equiv!;
   . exact nec! $ axiomK'! $ nec! $ and₂'! neg_equiv!;
 
-instance [System.S4 mΛ] : System.K4 mΛ where
+instance [System.S4 mH] : System.K4 mH where
 
 open provable_efq_of_provable_S4 in
-lemma provable_efq_of_provable_S4 [DecidableEq α] (h : 𝐈𝐧𝐭 ⊢! φ) : 𝐒𝟒 ⊢! φᵍ := by
+lemma provable_efq_of_provable_S4 [DecidableEq α] (h : (Hilbert.Int α) ⊢! φ) : (Hilbert.S4 α) ⊢! φᵍ := by
   induction h.some with
   | eaxm ih =>
     simp_all only [Set.mem_setOf_eq];
@@ -95,13 +95,13 @@ lemma provable_efq_of_provable_S4 [DecidableEq α] (h : 𝐈𝐧𝐭 ⊢! φ) : 
 end
 
 
-lemma dp_of_mdp [DecidableEq α] [ModalDisjunctive mΛ] [ModalCompanion iΛ mΛ] [System.S4 mΛ] : iΛ ⊢! φ ⋎ ψ → iΛ ⊢! φ ∨ iΛ ⊢! ψ := by
+lemma dp_of_mdp [DecidableEq α] [ModalDisjunctive mH] [ModalCompanion iH mH] [System.S4 mH] : iH ⊢! φ ⋎ ψ → iH ⊢! φ ∨ iH ⊢! ψ := by
     intro hpq;
-    have : mΛ ⊢! □φᵍ ⋎ □ψᵍ := or₃'''! (imply_left_or'! axiomTc_GTranslate!) (imply_right_or'! axiomTc_GTranslate!) (by simpa using ModalCompanion.companion.mp hpq);
+    have : mH ⊢! □φᵍ ⋎ □ψᵍ := or₃'''! (imply_left_or'! axiomTc_GTranslate!) (imply_right_or'! axiomTc_GTranslate!) (by simpa using ModalCompanion.companion.mp hpq);
     cases ModalDisjunctive.modal_disjunctive this with
     | inl h => left; exact ModalCompanion.companion.mpr h;
     | inr h => right; exact ModalCompanion.companion.mpr h;
 
-theorem disjunctive_of_modalDisjunctive [DecidableEq α] [ModalDisjunctive mΛ] [ModalCompanion iΛ mΛ] [System.S4 mΛ] : Disjunctive iΛ := ⟨dp_of_mdp (iΛ := iΛ) (mΛ := mΛ)⟩
+theorem disjunctive_of_modalDisjunctive [DecidableEq α] [ModalDisjunctive mH] [ModalCompanion iH mH] [System.S4 mH] : Disjunctive iH := ⟨dp_of_mdp (iH := iH) (mH := mH)⟩
 
 end LO.Modal
