Foundation/Modal/PLoN/Semantics.lean
@@ -175,7 +175,7 @@ protected lemma elim_contra : 𝔽 ⊧ (Axioms.ElimContra φ ψ) := by intro _ _
 end Formula.PLoN.ValidOnFrameClass
 
 
-def Hilbert.DefinesPLoNFrameClass (Λ : Hilbert α) (𝔽 : PLoN.FrameClass α) := ∀ {F : Frame α}, F ⊧* Λ.theorems ↔ F ∈ 𝔽
+def Hilbert.DefinesPLoNFrameClass (H : Hilbert α) (𝔽 : PLoN.FrameClass α) := ∀ {F : Frame α}, F ⊧* H.theorems ↔ F ∈ 𝔽
 
 namespace PLoN
 
@@ -188,11 +188,11 @@ lemma AllFrameClass.nonempty : (AllFrameClass.{_, 0} α).Nonempty := by
 
 open Formula
 
-lemma N_defines : 𝐍.DefinesPLoNFrameClass (AllFrameClass α) := by
+lemma N_defines : (Hilbert.N α).DefinesPLoNFrameClass (AllFrameClass α) := by
   intro F;
   simp [Hilbert.theorems, System.theory, PLoN.ValidOnFrame, PLoN.ValidOnModel];
   intro φ hp;
-  induction hp using Deduction.inducition_with_necOnly! with
+  induction hp using Hilbert.Deduction.inducition_with_necOnly! with
   | hMaxm h => simp at h;
   | hMdp ihpq ihp =>
     intro V w;
